WIP OneHot20

Risc0/Gadgets/OneHot20/Constraints/WeakestPresPart18.lean
@@ -8,53 +8,118 @@ namespace Risc0.OneHot20.Constraints.WP
 open MLIRNotation
 
 -- The state obtained by running Code.part18 on st
-def part18_state (st: State) : State := 
+def part18_state (st: State) : State :=
   
-        ((((st[felts][{ name := "%72" }] ←
-                Option.get! (State.felts st { name := "%69" }) +
-                  Option.get! (State.felts st { name := "%71" }))["%73"] ←ₛ
-              getImpl st { name := "data" } 0 19)[felts][{ name := "%74" }] ←
+        ((((st[felts][{ name := "%74" }] ←
+                Option.get! (State.felts st { name := "%73" }) *
+                  Option.get! (State.felts st { name := "%18" }))[felts][{ name := "%75" }] ←
+              Option.get! (State.felts st { name := "%72" }) +
+                Option.get! (State.felts st { name := "%73" }) *
+                  Option.get! (State.felts st { name := "%18" }))["%20"] ←ₛ
+            getImpl st { name := "code" } 0 0)[felts][{ name := "%76" }] ←
+          Option.get! (State.felts st { name := "%72" }) +
+              Option.get! (State.felts st { name := "%73" }) * Option.get! (State.felts st { name := "%18" }) -
             Option.get!
-                (State.felts
-                  ((st[felts][{ name := "%72" }] ←
-                      Option.get! (State.felts st { name := "%69" }) +
-                        Option.get! (State.felts st { name := "%71" }))["%73"] ←ₛ
-                    getImpl st { name := "data" } 0 19)
-                  { name := "%73" }) *
-              Option.get! (State.felts st { name := "%18" }))[felts][{ name := "%75" }] ←
-          Option.get! (State.felts st { name := "%69" }) + Option.get! (State.felts st { name := "%71" }) +
-            Option.get!
-                (State.felts
-                  ((st[felts][{ name := "%72" }] ←
-                      Option.get! (State.felts st { name := "%69" }) +
-                        Option.get! (State.felts st { name := "%71" }))["%73"] ←ₛ
-                    getImpl st { name := "data" } 0 19)
-                  { name := "%73" }) *
-              Option.get!
-                (State.felts st
-                  {
-                    name :=
-                      "%18" })) 
+              (State.felts
+                (((st[felts][{ name := "%74" }] ←
+                      Option.get! (State.felts st { name := "%73" }) *
+                        Option.get! (State.felts st { name := "%18" }))[felts][{ name := "%75" }] ←
+                    Option.get! (State.felts st { name := "%72" }) +
+                      Option.get! (State.felts st { name := "%73" }) *
+                        Option.get! (State.felts st { name := "%18" }))["%20"] ←ₛ
+                  getImpl st { name := "code" } 0 0)
+                { name := "%20" })) 
 
--- Run the whole program by using part18_state rather than Code.part18
+def part18_drops (st: State) : State :=
+  State.dropFelts (State.dropFelts (State.dropFelts (State.dropFelts (State.dropFelts (st) ⟨"%72"⟩) ⟨"%18"⟩) ⟨"%74"⟩) ⟨"%75"⟩) ⟨"%20"⟩
+
+-- Run the program from part18 onwards by using part18_state rather than Code.part18
 def part18_state_update (st: State): State :=
-  Γ (part18_state st) ⟦Code.part19; Code.part20; Code.part21; Code.part22; Code.part23; Code.part24; Code.part25; Code.part26; Code.part27; Code.part28; Code.part29; Code.part30; Code.part31; Code.part32; Code.part33; Code.part34; Code.part35; Code.part36; Code.part37; Code.part38; Code.part39⟧
+  Γ (part18_drops (part18_state st)) ⟦Code.part19;dropfelt ⟨"%76"⟩;Code.part20;dropfelt ⟨"%79"⟩;dropfelt ⟨"%80"⟩;dropfelt ⟨"%82"⟩;Code.part21;dropfelt ⟨"%21"⟩;dropfelt ⟨"%78"⟩;dropfelt ⟨"%83"⟩;dropfelt ⟨"%86"⟩;Code.part22;dropfelt ⟨"%22"⟩;dropfelt ⟨"%85"⟩;dropfelt ⟨"%87"⟩;dropfelt ⟨"%90"⟩;Code.part23;dropfelt ⟨"%25"⟩;dropfelt ⟨"%89"⟩;dropfelt ⟨"%91"⟩;dropfelt ⟨"%94"⟩;Code.part24;dropfelt ⟨"%28"⟩;dropfelt ⟨"%93"⟩;dropfelt ⟨"%95"⟩;dropfelt ⟨"%98"⟩;Code.part25;dropfelt ⟨"%31"⟩;dropfelt ⟨"%97"⟩;dropfelt ⟨"%99"⟩;dropfelt ⟨"%102"⟩;Code.part26;dropfelt ⟨"%34"⟩;dropfelt ⟨"%101"⟩;dropfelt ⟨"%103"⟩;dropfelt ⟨"%106"⟩;Code.part27;dropfelt ⟨"%37"⟩;dropfelt ⟨"%105"⟩;dropfelt ⟨"%107"⟩;dropfelt ⟨"%110"⟩;Code.part28;dropfelt ⟨"%40"⟩;dropfelt ⟨"%109"⟩;dropfelt ⟨"%111"⟩;dropfelt ⟨"%114"⟩;Code.part29;dropfelt ⟨"%43"⟩;dropfelt ⟨"%113"⟩;dropfelt ⟨"%115"⟩;dropfelt ⟨"%118"⟩;Code.part30;dropfelt ⟨"%46"⟩;dropfelt ⟨"%117"⟩;dropfelt ⟨"%119"⟩;dropfelt ⟨"%122"⟩;Code.part31;dropfelt ⟨"%49"⟩;dropfelt ⟨"%121"⟩;dropfelt ⟨"%123"⟩;dropfelt ⟨"%126"⟩;Code.part32;dropfelt ⟨"%52"⟩;dropfelt ⟨"%125"⟩;dropfelt ⟨"%127"⟩;dropfelt ⟨"%130"⟩;Code.part33;dropfelt ⟨"%55"⟩;dropfelt ⟨"%129"⟩;dropfelt ⟨"%131"⟩;dropfelt ⟨"%134"⟩;Code.part34;dropfelt ⟨"%58"⟩;dropfelt ⟨"%133"⟩;dropfelt ⟨"%135"⟩;dropfelt ⟨"%138"⟩;Code.part35;dropfelt ⟨"%61"⟩;dropfelt ⟨"%137"⟩;dropfelt ⟨"%139"⟩;dropfelt ⟨"%142"⟩;Code.part36;dropfelt ⟨"%64"⟩;dropfelt ⟨"%141"⟩;dropfelt ⟨"%143"⟩;dropfelt ⟨"%146"⟩;Code.part37;dropfelt ⟨"%67"⟩;dropfelt ⟨"%145"⟩;dropfelt ⟨"%147"⟩;dropfelt ⟨"%150"⟩;Code.part38;dropfelt ⟨"%70"⟩;dropfelt ⟨"%149"⟩;dropfelt ⟨"%151"⟩;dropfelt ⟨"%154"⟩;Code.part39;dropfelt ⟨"%19"⟩;dropfelt ⟨"%73"⟩;dropfelt ⟨"%77"⟩;dropfelt ⟨"%0"⟩;dropfelt ⟨"%81"⟩;dropfelt ⟨"%84"⟩;dropfelt ⟨"%88"⟩;dropfelt ⟨"%92"⟩;dropfelt ⟨"%96"⟩;dropfelt ⟨"%100"⟩;dropfelt ⟨"%104"⟩;dropfelt ⟨"%108"⟩;dropfelt ⟨"%112"⟩;dropfelt ⟨"%116"⟩;dropfelt ⟨"%120"⟩;dropfelt ⟨"%124"⟩;dropfelt ⟨"%128"⟩;dropfelt ⟨"%132"⟩;dropfelt ⟨"%136"⟩;dropfelt ⟨"%140"⟩;dropfelt ⟨"%144"⟩;dropfelt ⟨"%148"⟩;dropfelt ⟨"%152"⟩;dropfelt ⟨"%153"⟩;dropfelt ⟨"%155"⟩;dropfelt ⟨"%156"⟩;dropfelt ⟨"%157"⟩;dropfelt ⟨"%158"⟩;dropfelt ⟨"%159"⟩⟧
 
 -- Prove that substituting part18_state for Code.part18 produces the same result
 lemma part18_wp {st : State} :
-  Code.getReturn (MLIR.runProgram (Code.part18; Code.part19; Code.part20; Code.part21; Code.part22; Code.part23; Code.part24; Code.part25; Code.part26; Code.part27; Code.part28; Code.part29; Code.part30; Code.part31; Code.part32; Code.part33; Code.part34; Code.part35; Code.part36; Code.part37; Code.part38; Code.part39) st) ↔
+  Code.getReturn (MLIR.runProgram (Code.part18;dropfelt ⟨"%72"⟩;dropfelt ⟨"%18"⟩;dropfelt ⟨"%74"⟩;dropfelt ⟨"%75"⟩;dropfelt ⟨"%20"⟩;Code.part19;dropfelt ⟨"%76"⟩;Code.part20;dropfelt ⟨"%79"⟩;dropfelt ⟨"%80"⟩;dropfelt ⟨"%82"⟩;Code.part21;dropfelt ⟨"%21"⟩;dropfelt ⟨"%78"⟩;dropfelt ⟨"%83"⟩;dropfelt ⟨"%86"⟩;Code.part22;dropfelt ⟨"%22"⟩;dropfelt ⟨"%85"⟩;dropfelt ⟨"%87"⟩;dropfelt ⟨"%90"⟩;Code.part23;dropfelt ⟨"%25"⟩;dropfelt ⟨"%89"⟩;dropfelt ⟨"%91"⟩;dropfelt ⟨"%94"⟩;Code.part24;dropfelt ⟨"%28"⟩;dropfelt ⟨"%93"⟩;dropfelt ⟨"%95"⟩;dropfelt ⟨"%98"⟩;Code.part25;dropfelt ⟨"%31"⟩;dropfelt ⟨"%97"⟩;dropfelt ⟨"%99"⟩;dropfelt ⟨"%102"⟩;Code.part26;dropfelt ⟨"%34"⟩;dropfelt ⟨"%101"⟩;dropfelt ⟨"%103"⟩;dropfelt ⟨"%106"⟩;Code.part27;dropfelt ⟨"%37"⟩;dropfelt ⟨"%105"⟩;dropfelt ⟨"%107"⟩;dropfelt ⟨"%110"⟩;Code.part28;dropfelt ⟨"%40"⟩;dropfelt ⟨"%109"⟩;dropfelt ⟨"%111"⟩;dropfelt ⟨"%114"⟩;Code.part29;dropfelt ⟨"%43"⟩;dropfelt ⟨"%113"⟩;dropfelt ⟨"%115"⟩;dropfelt ⟨"%118"⟩;Code.part30;dropfelt ⟨"%46"⟩;dropfelt ⟨"%117"⟩;dropfelt ⟨"%119"⟩;dropfelt ⟨"%122"⟩;Code.part31;dropfelt ⟨"%49"⟩;dropfelt ⟨"%121"⟩;dropfelt ⟨"%123"⟩;dropfelt ⟨"%126"⟩;Code.part32;dropfelt ⟨"%52"⟩;dropfelt ⟨"%125"⟩;dropfelt ⟨"%127"⟩;dropfelt ⟨"%130"⟩;Code.part33;dropfelt ⟨"%55"⟩;dropfelt ⟨"%129"⟩;dropfelt ⟨"%131"⟩;dropfelt ⟨"%134"⟩;Code.part34;dropfelt ⟨"%58"⟩;dropfelt ⟨"%133"⟩;dropfelt ⟨"%135"⟩;dropfelt ⟨"%138"⟩;Code.part35;dropfelt ⟨"%61"⟩;dropfelt ⟨"%137"⟩;dropfelt ⟨"%139"⟩;dropfelt ⟨"%142"⟩;Code.part36;dropfelt ⟨"%64"⟩;dropfelt ⟨"%141"⟩;dropfelt ⟨"%143"⟩;dropfelt ⟨"%146"⟩;Code.part37;dropfelt ⟨"%67"⟩;dropfelt ⟨"%145"⟩;dropfelt ⟨"%147"⟩;dropfelt ⟨"%150"⟩;Code.part38;dropfelt ⟨"%70"⟩;dropfelt ⟨"%149"⟩;dropfelt ⟨"%151"⟩;dropfelt ⟨"%154"⟩;Code.part39;dropfelt ⟨"%19"⟩;dropfelt ⟨"%73"⟩;dropfelt ⟨"%77"⟩;dropfelt ⟨"%0"⟩;dropfelt ⟨"%81"⟩;dropfelt ⟨"%84"⟩;dropfelt ⟨"%88"⟩;dropfelt ⟨"%92"⟩;dropfelt ⟨"%96"⟩;dropfelt ⟨"%100"⟩;dropfelt ⟨"%104"⟩;dropfelt ⟨"%108"⟩;dropfelt ⟨"%112"⟩;dropfelt ⟨"%116"⟩;dropfelt ⟨"%120"⟩;dropfelt ⟨"%124"⟩;dropfelt ⟨"%128"⟩;dropfelt ⟨"%132"⟩;dropfelt ⟨"%136"⟩;dropfelt ⟨"%140"⟩;dropfelt ⟨"%144"⟩;dropfelt ⟨"%148"⟩;dropfelt ⟨"%152"⟩;dropfelt ⟨"%153"⟩;dropfelt ⟨"%155"⟩;dropfelt ⟨"%156"⟩;dropfelt ⟨"%157"⟩;dropfelt ⟨"%158"⟩;dropfelt ⟨"%159"⟩) st) ↔
   Code.getReturn (part18_state_update st) := by
   unfold MLIR.runProgram; simp only
-  generalize eq : (Code.part19; Code.part20; Code.part21; Code.part22; Code.part23; Code.part24; Code.part25; Code.part26; Code.part27; Code.part28; Code.part29; Code.part30; Code.part31; Code.part32; Code.part33; Code.part34; Code.part35; Code.part36; Code.part37; Code.part38; Code.part39) = prog
+  generalize eq : (dropfelt ⟨"%72"⟩;dropfelt ⟨"%18"⟩;dropfelt ⟨"%74"⟩;dropfelt ⟨"%75"⟩;dropfelt ⟨"%20"⟩;Code.part19;dropfelt ⟨"%76"⟩;Code.part20;dropfelt ⟨"%79"⟩;dropfelt ⟨"%80"⟩;dropfelt ⟨"%82"⟩;Code.part21;dropfelt ⟨"%21"⟩;dropfelt ⟨"%78"⟩;dropfelt ⟨"%83"⟩;dropfelt ⟨"%86"⟩;Code.part22;dropfelt ⟨"%22"⟩;dropfelt ⟨"%85"⟩;dropfelt ⟨"%87"⟩;dropfelt ⟨"%90"⟩;Code.part23;dropfelt ⟨"%25"⟩;dropfelt ⟨"%89"⟩;dropfelt ⟨"%91"⟩;dropfelt ⟨"%94"⟩;Code.part24;dropfelt ⟨"%28"⟩;dropfelt ⟨"%93"⟩;dropfelt ⟨"%95"⟩;dropfelt ⟨"%98"⟩;Code.part25;dropfelt ⟨"%31"⟩;dropfelt ⟨"%97"⟩;dropfelt ⟨"%99"⟩;dropfelt ⟨"%102"⟩;Code.part26;dropfelt ⟨"%34"⟩;dropfelt ⟨"%101"⟩;dropfelt ⟨"%103"⟩;dropfelt ⟨"%106"⟩;Code.part27;dropfelt ⟨"%37"⟩;dropfelt ⟨"%105"⟩;dropfelt ⟨"%107"⟩;dropfelt ⟨"%110"⟩;Code.part28;dropfelt ⟨"%40"⟩;dropfelt ⟨"%109"⟩;dropfelt ⟨"%111"⟩;dropfelt ⟨"%114"⟩;Code.part29;dropfelt ⟨"%43"⟩;dropfelt ⟨"%113"⟩;dropfelt ⟨"%115"⟩;dropfelt ⟨"%118"⟩;Code.part30;dropfelt ⟨"%46"⟩;dropfelt ⟨"%117"⟩;dropfelt ⟨"%119"⟩;dropfelt ⟨"%122"⟩;Code.part31;dropfelt ⟨"%49"⟩;dropfelt ⟨"%121"⟩;dropfelt ⟨"%123"⟩;dropfelt ⟨"%126"⟩;Code.part32;dropfelt ⟨"%52"⟩;dropfelt ⟨"%125"⟩;dropfelt ⟨"%127"⟩;dropfelt ⟨"%130"⟩;Code.part33;dropfelt ⟨"%55"⟩;dropfelt ⟨"%129"⟩;dropfelt ⟨"%131"⟩;dropfelt ⟨"%134"⟩;Code.part34;dropfelt ⟨"%58"⟩;dropfelt ⟨"%133"⟩;dropfelt ⟨"%135"⟩;dropfelt ⟨"%138"⟩;Code.part35;dropfelt ⟨"%61"⟩;dropfelt ⟨"%137"⟩;dropfelt ⟨"%139"⟩;dropfelt ⟨"%142"⟩;Code.part36;dropfelt ⟨"%64"⟩;dropfelt ⟨"%141"⟩;dropfelt ⟨"%143"⟩;dropfelt ⟨"%146"⟩;Code.part37;dropfelt ⟨"%67"⟩;dropfelt ⟨"%145"⟩;dropfelt ⟨"%147"⟩;dropfelt ⟨"%150"⟩;Code.part38;dropfelt ⟨"%70"⟩;dropfelt ⟨"%149"⟩;dropfelt ⟨"%151"⟩;dropfelt ⟨"%154"⟩;Code.part39;dropfelt ⟨"%19"⟩;dropfelt ⟨"%73"⟩;dropfelt ⟨"%77"⟩;dropfelt ⟨"%0"⟩;dropfelt ⟨"%81"⟩;dropfelt ⟨"%84"⟩;dropfelt ⟨"%88"⟩;dropfelt ⟨"%92"⟩;dropfelt ⟨"%96"⟩;dropfelt ⟨"%100"⟩;dropfelt ⟨"%104"⟩;dropfelt ⟨"%108"⟩;dropfelt ⟨"%112"⟩;dropfelt ⟨"%116"⟩;dropfelt ⟨"%120"⟩;dropfelt ⟨"%124"⟩;dropfelt ⟨"%128"⟩;dropfelt ⟨"%132"⟩;dropfelt ⟨"%136"⟩;dropfelt ⟨"%140"⟩;dropfelt ⟨"%144"⟩;dropfelt ⟨"%148"⟩;dropfelt ⟨"%152"⟩;dropfelt ⟨"%153"⟩;dropfelt ⟨"%155"⟩;dropfelt ⟨"%156"⟩;dropfelt ⟨"%157"⟩;dropfelt ⟨"%158"⟩;dropfelt ⟨"%159"⟩) = prog
   unfold Code.part18
   MLIR
-  unfold part18_state_update part18_state
   rewrite [←eq]
+  rewrite [MLIR.run_seq_def,MLIR.run_dropfelt, MLIR.run_seq_def,MLIR.run_dropfelt, MLIR.run_seq_def,MLIR.run_dropfelt, MLIR.run_seq_def,MLIR.run_dropfelt, MLIR.run_seq_def,MLIR.run_dropfelt]
+  unfold part18_state_update part18_drops part18_state
   rfl
 
 lemma part18_updates_opaque {st : State} : 
   Code.getReturn (part17_state_update st) ↔
-  Code.getReturn (part18_state_update (part17_state st)) := by
+  Code.getReturn (part18_state_update (part17_drops (part17_state st))) := by
   simp [part17_state_update, part18_wp]
+
+lemma part18_cumulative_wp {x0 y0 y1 y2 y3 y4 y5 y6 y7 y8 y9 y10 y11 y12 y13 y14 y15 y16 y17 y18 y19: Felt} :
+  Code.run (start_state [x0] ([y0,y1,y2,y3,y4,y5,y6,y7,y8,y9,y10,y11,y12,y13,y14,y15,y16,y17,y18,y19])) ↔
+  Code.getReturn
+      (part18_state_update
+        (((((((((((((((((((((({
+                                                      buffers :=
+                                                        ((fun x => Map.empty x)[{ name := "data" }] ←ₘ
+                                                            [[some y0, some y1, some y2, some y3, some y4, some y5,
+                                                                some y6, some y7, some y8, some y9, some y10, some y11,
+                                                                some y12, some y13, some y14, some y15, some y16,
+                                                                some y17, some y18, some y19]])[{ name := "code" }] ←ₘ
+                                                          [[some x0]],
+                                                      bufferWidths :=
+                                                        ((fun x => Map.empty x)[{ name := "data" }] ←ₘ
+                                                            20)[{ name := "code" }] ←ₘ
+                                                          1,
+                                                      constraints := [], cycle := 0, felts := Map.empty,
+                                                      isFailed := false, props := Map.empty,
+                                                      vars :=
+                                                        [{ name := "code" },
+                                                          { name := "data" }] }[props][{ name := "%19" }] ←
+                                                    True)[felts][{ name := "%22" }] ←
+                                                  y2)[felts][{ name := "%21" }] ←
+                                                y1)[felts][{ name := "%25" }] ←
+                                              y3)[felts][{ name := "%28" }] ←
+                                            y4)[felts][{ name := "%31" }] ←
+                                          y5)[felts][{ name := "%34" }] ←
+                                        y6)[felts][{ name := "%37" }] ←
+                                      y7)[felts][{ name := "%40" }] ←
+                                    y8)[felts][{ name := "%43" }] ←
+                                  y9)[felts][{ name := "%46" }] ←
+                                y10)[felts][{ name := "%49" }] ←
+                              y11)[felts][{ name := "%52" }] ←
+                            y12)[felts][{ name := "%55" }] ←
+                          y13)[felts][{ name := "%58" }] ←
+                        y14)[felts][{ name := "%61" }] ←
+                      y15)[felts][{ name := "%64" }] ←
+                    y16)[felts][{ name := "%67" }] ←
+                  y17)[felts][{ name := "%70" }] ←
+                y18)[felts][{ name := "%72" }] ←
+              y1 + y2 * 2 + y3 * 3 + y4 * 4 + y5 * 5 + y6 * 6 + y7 * 7 + y8 * 8 + y9 * 9 + y10 * 10 + y11 * 11 +
+                            y12 * 12 +
+                          y13 * 13 +
+                        y14 * 14 +
+                      y15 * 15 +
+                    y16 * 16 +
+                  y17 * 17 +
+                y18 * 18)[felts][{ name := "%18" }] ←
+            19)[felts][{ name := "%73" }] ←
+          y19))  := by
+    rewrite [part17_cumulative_wp]
+    rewrite [part18_updates_opaque]
+    unfold part17_state
+    MLIR_states_updates
+    -- 0 withEqZeros
+    -- rewrite [withEqZero_def]
+    -- MLIR_states_updates
+    unfold part17_drops
+    -- 3 drops
+    simp only [State.drop_update_swap, State.drop_update_same, State.drop_updateProps_swap]
+    rewrite [State.dropFelts]
+    simp only [State.dropFelts_buffers, State.dropFelts_bufferWidths, State.dropFelts_constraints, State.dropFelts_cycle, State.dropFelts_felts, State.dropFelts_isFailed, State.dropFelts_props, State.dropFelts_vars]
+    simp only [Map.drop_base, ne_eq, Map.update_drop_swap, Map.update_drop]
+    -- 0 sets
+    -- rewrite [Map.drop_of_updates]
+    -- simp only [Map.drop_base, ne_eq, Map.update_drop_swap, Map.update_drop]
 
 end Risc0.OneHot20.Constraints.WP
