Risc0/Gadgets/OneHot20/Constraints/WeakestPresPart32.lean
@@ -8,7 +8,7 @@ namespace Risc0.OneHot20.Constraints.WP
 open MLIRNotation
 
 -- The state obtained by running Code.part32 on st
-def part32_state (st: State) : State := 
+def part32_state (st: State) : State :=
   
         ((((st[props][{ name := "%128" }] ←
                 (Option.get! (State.props st { name := "%124" }) ∧
@@ -18,32 +18,321 @@ def part32_state (st: State) : State :=
             Option.get! (State.felts st { name := "%0" }) -
               Option.get! (State.felts st { name := "%55" }))[felts][{ name := "%131" }] ←
           Option.get! (State.felts st { name := "%55" }) *
-            (Option.get! (State.felts st { name := "%0" }) -
-              Option.get!
-                (State.felts st
-                  {
-                    name :=
-                      "%55" }))) 
+            (Option.get! (State.felts st { name := "%0" }) - Option.get! (State.felts st { name := "%55" }))) 
 
--- Run the whole program by using part32_state rather than Code.part32
+def part32_drops (st: State) : State :=
+  State.dropFelts (State.dropFelts (State.dropFelts (State.dropFelts (st) ⟨"%52"⟩) ⟨"%125"⟩) ⟨"%127"⟩) ⟨"%130"⟩
+
+-- Run the program from part32 onwards by using part32_state rather than Code.part32
 def part32_state_update (st: State): State :=
-  Γ (part32_state st) ⟦Code.part33; Code.part34; Code.part35; Code.part36; Code.part37; Code.part38; Code.part39⟧
+  Γ (part32_drops (part32_state st)) ⟦Code.part33;dropfelt ⟨"%55"⟩;dropfelt ⟨"%129"⟩;dropfelt ⟨"%131"⟩;dropfelt ⟨"%134"⟩;Code.part34;dropfelt ⟨"%58"⟩;dropfelt ⟨"%133"⟩;dropfelt ⟨"%135"⟩;dropfelt ⟨"%138"⟩;Code.part35;dropfelt ⟨"%61"⟩;dropfelt ⟨"%137"⟩;dropfelt ⟨"%139"⟩;dropfelt ⟨"%142"⟩;Code.part36;dropfelt ⟨"%64"⟩;dropfelt ⟨"%141"⟩;dropfelt ⟨"%143"⟩;dropfelt ⟨"%146"⟩;Code.part37;dropfelt ⟨"%67"⟩;dropfelt ⟨"%145"⟩;dropfelt ⟨"%147"⟩;dropfelt ⟨"%150"⟩;Code.part38;dropfelt ⟨"%70"⟩;dropfelt ⟨"%149"⟩;dropfelt ⟨"%151"⟩;dropfelt ⟨"%154"⟩;Code.part39;dropfelt ⟨"%19"⟩;dropfelt ⟨"%73"⟩;dropfelt ⟨"%77"⟩;dropfelt ⟨"%0"⟩;dropfelt ⟨"%81"⟩;dropfelt ⟨"%84"⟩;dropfelt ⟨"%88"⟩;dropfelt ⟨"%92"⟩;dropfelt ⟨"%96"⟩;dropfelt ⟨"%100"⟩;dropfelt ⟨"%104"⟩;dropfelt ⟨"%108"⟩;dropfelt ⟨"%112"⟩;dropfelt ⟨"%116"⟩;dropfelt ⟨"%120"⟩;dropfelt ⟨"%124"⟩;dropfelt ⟨"%128"⟩;dropfelt ⟨"%132"⟩;dropfelt ⟨"%136"⟩;dropfelt ⟨"%140"⟩;dropfelt ⟨"%144"⟩;dropfelt ⟨"%148"⟩;dropfelt ⟨"%152"⟩;dropfelt ⟨"%153"⟩;dropfelt ⟨"%155"⟩;dropfelt ⟨"%156"⟩;dropfelt ⟨"%157"⟩;dropfelt ⟨"%158"⟩;dropfelt ⟨"%159"⟩⟧
 
 -- Prove that substituting part32_state for Code.part32 produces the same result
 lemma part32_wp {st : State} :
-  Code.getReturn (MLIR.runProgram (Code.part32; Code.part33; Code.part34; Code.part35; Code.part36; Code.part37; Code.part38; Code.part39) st) ↔
+  Code.getReturn (MLIR.runProgram (Code.part32;dropfelt ⟨"%52"⟩;dropfelt ⟨"%125"⟩;dropfelt ⟨"%127"⟩;dropfelt ⟨"%130"⟩;Code.part33;dropfelt ⟨"%55"⟩;dropfelt ⟨"%129"⟩;dropfelt ⟨"%131"⟩;dropfelt ⟨"%134"⟩;Code.part34;dropfelt ⟨"%58"⟩;dropfelt ⟨"%133"⟩;dropfelt ⟨"%135"⟩;dropfelt ⟨"%138"⟩;Code.part35;dropfelt ⟨"%61"⟩;dropfelt ⟨"%137"⟩;dropfelt ⟨"%139"⟩;dropfelt ⟨"%142"⟩;Code.part36;dropfelt ⟨"%64"⟩;dropfelt ⟨"%141"⟩;dropfelt ⟨"%143"⟩;dropfelt ⟨"%146"⟩;Code.part37;dropfelt ⟨"%67"⟩;dropfelt ⟨"%145"⟩;dropfelt ⟨"%147"⟩;dropfelt ⟨"%150"⟩;Code.part38;dropfelt ⟨"%70"⟩;dropfelt ⟨"%149"⟩;dropfelt ⟨"%151"⟩;dropfelt ⟨"%154"⟩;Code.part39;dropfelt ⟨"%19"⟩;dropfelt ⟨"%73"⟩;dropfelt ⟨"%77"⟩;dropfelt ⟨"%0"⟩;dropfelt ⟨"%81"⟩;dropfelt ⟨"%84"⟩;dropfelt ⟨"%88"⟩;dropfelt ⟨"%92"⟩;dropfelt ⟨"%96"⟩;dropfelt ⟨"%100"⟩;dropfelt ⟨"%104"⟩;dropfelt ⟨"%108"⟩;dropfelt ⟨"%112"⟩;dropfelt ⟨"%116"⟩;dropfelt ⟨"%120"⟩;dropfelt ⟨"%124"⟩;dropfelt ⟨"%128"⟩;dropfelt ⟨"%132"⟩;dropfelt ⟨"%136"⟩;dropfelt ⟨"%140"⟩;dropfelt ⟨"%144"⟩;dropfelt ⟨"%148"⟩;dropfelt ⟨"%152"⟩;dropfelt ⟨"%153"⟩;dropfelt ⟨"%155"⟩;dropfelt ⟨"%156"⟩;dropfelt ⟨"%157"⟩;dropfelt ⟨"%158"⟩;dropfelt ⟨"%159"⟩) st) ↔
   Code.getReturn (part32_state_update st) := by
   unfold MLIR.runProgram; simp only
-  generalize eq : (Code.part33; Code.part34; Code.part35; Code.part36; Code.part37; Code.part38; Code.part39) = prog
+  generalize eq : (dropfelt ⟨"%52"⟩;dropfelt ⟨"%125"⟩;dropfelt ⟨"%127"⟩;dropfelt ⟨"%130"⟩;Code.part33;dropfelt ⟨"%55"⟩;dropfelt ⟨"%129"⟩;dropfelt ⟨"%131"⟩;dropfelt ⟨"%134"⟩;Code.part34;dropfelt ⟨"%58"⟩;dropfelt ⟨"%133"⟩;dropfelt ⟨"%135"⟩;dropfelt ⟨"%138"⟩;Code.part35;dropfelt ⟨"%61"⟩;dropfelt ⟨"%137"⟩;dropfelt ⟨"%139"⟩;dropfelt ⟨"%142"⟩;Code.part36;dropfelt ⟨"%64"⟩;dropfelt ⟨"%141"⟩;dropfelt ⟨"%143"⟩;dropfelt ⟨"%146"⟩;Code.part37;dropfelt ⟨"%67"⟩;dropfelt ⟨"%145"⟩;dropfelt ⟨"%147"⟩;dropfelt ⟨"%150"⟩;Code.part38;dropfelt ⟨"%70"⟩;dropfelt ⟨"%149"⟩;dropfelt ⟨"%151"⟩;dropfelt ⟨"%154"⟩;Code.part39;dropfelt ⟨"%19"⟩;dropfelt ⟨"%73"⟩;dropfelt ⟨"%77"⟩;dropfelt ⟨"%0"⟩;dropfelt ⟨"%81"⟩;dropfelt ⟨"%84"⟩;dropfelt ⟨"%88"⟩;dropfelt ⟨"%92"⟩;dropfelt ⟨"%96"⟩;dropfelt ⟨"%100"⟩;dropfelt ⟨"%104"⟩;dropfelt ⟨"%108"⟩;dropfelt ⟨"%112"⟩;dropfelt ⟨"%116"⟩;dropfelt ⟨"%120"⟩;dropfelt ⟨"%124"⟩;dropfelt ⟨"%128"⟩;dropfelt ⟨"%132"⟩;dropfelt ⟨"%136"⟩;dropfelt ⟨"%140"⟩;dropfelt ⟨"%144"⟩;dropfelt ⟨"%148"⟩;dropfelt ⟨"%152"⟩;dropfelt ⟨"%153"⟩;dropfelt ⟨"%155"⟩;dropfelt ⟨"%156"⟩;dropfelt ⟨"%157"⟩;dropfelt ⟨"%158"⟩;dropfelt ⟨"%159"⟩) = prog
   unfold Code.part32
   MLIR
-  unfold part32_state_update part32_state
   rewrite [←eq]
+  rewrite [MLIR.run_seq_def,MLIR.run_dropfelt, MLIR.run_seq_def,MLIR.run_dropfelt, MLIR.run_seq_def,MLIR.run_dropfelt, MLIR.run_seq_def,MLIR.run_dropfelt]
+  unfold part32_state_update part32_drops part32_state
   rfl
 
 lemma part32_updates_opaque {st : State} : 
   Code.getReturn (part31_state_update st) ↔
-  Code.getReturn (part32_state_update (part31_state st)) := by
+  Code.getReturn (part32_state_update (part31_drops (part31_state st))) := by
   simp [part31_state_update, part32_wp]
+
+lemma part32_cumulative_wp {x0 y0 y1 y2 y3 y4 y5 y6 y7 y8 y9 y10 y11 y12 y13 y14 y15 y16 y17 y18 y19: Felt} :
+  Code.run (start_state [x0] ([y0,y1,y2,y3,y4,y5,y6,y7,y8,y9,y10,y11,y12,y13,y14,y15,y16,y17,y18,y19])) ↔
+  Code.getReturn
+      (part32_state_update
+        ((((((((((((((((((((((((({
+                                                            buffers :=
+                                                              ((fun x => Map.empty x)[{ name := "data" }] ←ₘ
+                                                                  [[some y0, some y1, some y2, some y3, some y4,
+                                                                      some y5, some y6, some y7, some y8, some y9,
+                                                                      some y10, some y11, some y12, some y13, some y14,
+                                                                      some y15, some y16, some y17, some y18,
+                                                                      some y19]])[{ name := "code" }] ←ₘ
+                                                                [[some x0]],
+                                                            bufferWidths :=
+                                                              ((fun x => Map.empty x)[{ name := "data" }] ←ₘ
+                                                                  20)[{ name := "code" }] ←ₘ
+                                                                1,
+                                                            constraints := [], cycle := 0, felts := Map.empty,
+                                                            isFailed := false, props := Map.empty,
+                                                            vars :=
+                                                              [{ name := "code" },
+                                                                { name := "data" }] }[props][{ name := "%19" }] ←
+                                                          True)[felts][{ name := "%52" }] ←
+                                                        y12)[felts][{ name := "%55" }] ←
+                                                      y13)[felts][{ name := "%58" }] ←
+                                                    y14)[felts][{ name := "%61" }] ←
+                                                  y15)[felts][{ name := "%64" }] ←
+                                                y16)[felts][{ name := "%67" }] ←
+                                              y17)[felts][{ name := "%70" }] ←
+                                            y18)[felts][{ name := "%73" }] ←
+                                          y19)[props][{ name := "%77" }] ←
+                                        y1 + y2 * 2 + y3 * 3 + y4 * 4 + y5 * 5 + y6 * 6 + y7 * 7 + y8 * 8 + y9 * 9 +
+                                                                y10 * 10 +
+                                                              y11 * 11 +
+                                                            y12 * 12 +
+                                                          y13 * 13 +
+                                                        y14 * 14 +
+                                                      y15 * 15 +
+                                                    y16 * 16 +
+                                                  y17 * 17 +
+                                                y18 * 18 +
+                                              y19 * 19 -
+                                            x0 =
+                                          0)[felts][{ name := "%0" }] ←
+                                      1)[props][{ name := "%81" }] ←
+                                    (y1 + y2 * 2 + y3 * 3 + y4 * 4 + y5 * 5 + y6 * 6 + y7 * 7 + y8 * 8 + y9 * 9 +
+                                                              y10 * 10 +
+                                                            y11 * 11 +
+                                                          y12 * 12 +
+                                                        y13 * 13 +
+                                                      y14 * 14 +
+                                                    y15 * 15 +
+                                                  y16 * 16 +
+                                                y17 * 17 +
+                                              y18 * 18 +
+                                            y19 * 19 -
+                                          x0 =
+                                        0 ∧
+                                      (y0 = 0 ∨ 1 - y0 = 0)))[props][{ name := "%84" }] ←
+                                  ((y1 + y2 * 2 + y3 * 3 + y4 * 4 + y5 * 5 + y6 * 6 + y7 * 7 + y8 * 8 + y9 * 9 +
+                                                              y10 * 10 +
+                                                            y11 * 11 +
+                                                          y12 * 12 +
+                                                        y13 * 13 +
+                                                      y14 * 14 +
+                                                    y15 * 15 +
+                                                  y16 * 16 +
+                                                y17 * 17 +
+                                              y18 * 18 +
+                                            y19 * 19 -
+                                          x0 =
+                                        0 ∧
+                                      (y0 = 0 ∨ 1 - y0 = 0)) ∧
+                                    (y1 = 0 ∨ 1 - y1 = 0)))[props][{ name := "%88" }] ←
+                                (((y1 + y2 * 2 + y3 * 3 + y4 * 4 + y5 * 5 + y6 * 6 + y7 * 7 + y8 * 8 + y9 * 9 +
+                                                              y10 * 10 +
+                                                            y11 * 11 +
+                                                          y12 * 12 +
+                                                        y13 * 13 +
+                                                      y14 * 14 +
+                                                    y15 * 15 +
+                                                  y16 * 16 +
+                                                y17 * 17 +
+                                              y18 * 18 +
+                                            y19 * 19 -
+                                          x0 =
+                                        0 ∧
+                                      (y0 = 0 ∨ 1 - y0 = 0)) ∧
+                                    (y1 = 0 ∨ 1 - y1 = 0)) ∧
+                                  (y2 = 0 ∨ 1 - y2 = 0)))[props][{ name := "%92" }] ←
+                              ((((y1 + y2 * 2 + y3 * 3 + y4 * 4 + y5 * 5 + y6 * 6 + y7 * 7 + y8 * 8 + y9 * 9 +
+                                                              y10 * 10 +
+                                                            y11 * 11 +
+                                                          y12 * 12 +
+                                                        y13 * 13 +
+                                                      y14 * 14 +
+                                                    y15 * 15 +
+                                                  y16 * 16 +
+                                                y17 * 17 +
+                                              y18 * 18 +
+                                            y19 * 19 -
+                                          x0 =
+                                        0 ∧
+                                      (y0 = 0 ∨ 1 - y0 = 0)) ∧
+                                    (y1 = 0 ∨ 1 - y1 = 0)) ∧
+                                  (y2 = 0 ∨ 1 - y2 = 0)) ∧
+                                (y3 = 0 ∨ 1 - y3 = 0)))[props][{ name := "%96" }] ←
+                            (((((y1 + y2 * 2 + y3 * 3 + y4 * 4 + y5 * 5 + y6 * 6 + y7 * 7 + y8 * 8 + y9 * 9 + y10 * 10 +
+                                                            y11 * 11 +
+                                                          y12 * 12 +
+                                                        y13 * 13 +
+                                                      y14 * 14 +
+                                                    y15 * 15 +
+                                                  y16 * 16 +
+                                                y17 * 17 +
+                                              y18 * 18 +
+                                            y19 * 19 -
+                                          x0 =
+                                        0 ∧
+                                      (y0 = 0 ∨ 1 - y0 = 0)) ∧
+                                    (y1 = 0 ∨ 1 - y1 = 0)) ∧
+                                  (y2 = 0 ∨ 1 - y2 = 0)) ∧
+                                (y3 = 0 ∨ 1 - y3 = 0)) ∧
+                              (y4 = 0 ∨ 1 - y4 = 0)))[props][{ name := "%100" }] ←
+                          ((((((y1 + y2 * 2 + y3 * 3 + y4 * 4 + y5 * 5 + y6 * 6 + y7 * 7 + y8 * 8 + y9 * 9 + y10 * 10 +
+                                                            y11 * 11 +
+                                                          y12 * 12 +
+                                                        y13 * 13 +
+                                                      y14 * 14 +
+                                                    y15 * 15 +
+                                                  y16 * 16 +
+                                                y17 * 17 +
+                                              y18 * 18 +
+                                            y19 * 19 -
+                                          x0 =
+                                        0 ∧
+                                      (y0 = 0 ∨ 1 - y0 = 0)) ∧
+                                    (y1 = 0 ∨ 1 - y1 = 0)) ∧
+                                  (y2 = 0 ∨ 1 - y2 = 0)) ∧
+                                (y3 = 0 ∨ 1 - y3 = 0)) ∧
+                              (y4 = 0 ∨ 1 - y4 = 0)) ∧
+                            (y5 = 0 ∨ 1 - y5 = 0)))[props][{ name := "%104" }] ←
+                        (((((((y1 + y2 * 2 + y3 * 3 + y4 * 4 + y5 * 5 + y6 * 6 + y7 * 7 + y8 * 8 + y9 * 9 + y10 * 10 +
+                                                            y11 * 11 +
+                                                          y12 * 12 +
+                                                        y13 * 13 +
+                                                      y14 * 14 +
+                                                    y15 * 15 +
+                                                  y16 * 16 +
+                                                y17 * 17 +
+                                              y18 * 18 +
+                                            y19 * 19 -
+                                          x0 =
+                                        0 ∧
+                                      (y0 = 0 ∨ 1 - y0 = 0)) ∧
+                                    (y1 = 0 ∨ 1 - y1 = 0)) ∧
+                                  (y2 = 0 ∨ 1 - y2 = 0)) ∧
+                                (y3 = 0 ∨ 1 - y3 = 0)) ∧
+                              (y4 = 0 ∨ 1 - y4 = 0)) ∧
+                            (y5 = 0 ∨ 1 - y5 = 0)) ∧
+                          (y6 = 0 ∨ 1 - y6 = 0)))[props][{ name := "%108" }] ←
+                      ((((((((y1 + y2 * 2 + y3 * 3 + y4 * 4 + y5 * 5 + y6 * 6 + y7 * 7 + y8 * 8 + y9 * 9 + y10 * 10 +
+                                                            y11 * 11 +
+                                                          y12 * 12 +
+                                                        y13 * 13 +
+                                                      y14 * 14 +
+                                                    y15 * 15 +
+                                                  y16 * 16 +
+                                                y17 * 17 +
+                                              y18 * 18 +
+                                            y19 * 19 -
+                                          x0 =
+                                        0 ∧
+                                      (y0 = 0 ∨ 1 - y0 = 0)) ∧
+                                    (y1 = 0 ∨ 1 - y1 = 0)) ∧
+                                  (y2 = 0 ∨ 1 - y2 = 0)) ∧
+                                (y3 = 0 ∨ 1 - y3 = 0)) ∧
+                              (y4 = 0 ∨ 1 - y4 = 0)) ∧
+                            (y5 = 0 ∨ 1 - y5 = 0)) ∧
+                          (y6 = 0 ∨ 1 - y6 = 0)) ∧
+                        (y7 = 0 ∨ 1 - y7 = 0)))[props][{ name := "%112" }] ←
+                    (((((((((y1 + y2 * 2 + y3 * 3 + y4 * 4 + y5 * 5 + y6 * 6 + y7 * 7 + y8 * 8 + y9 * 9 + y10 * 10 +
+                                                            y11 * 11 +
+                                                          y12 * 12 +
+                                                        y13 * 13 +
+                                                      y14 * 14 +
+                                                    y15 * 15 +
+                                                  y16 * 16 +
+                                                y17 * 17 +
+                                              y18 * 18 +
+                                            y19 * 19 -
+                                          x0 =
+                                        0 ∧
+                                      (y0 = 0 ∨ 1 - y0 = 0)) ∧
+                                    (y1 = 0 ∨ 1 - y1 = 0)) ∧
+                                  (y2 = 0 ∨ 1 - y2 = 0)) ∧
+                                (y3 = 0 ∨ 1 - y3 = 0)) ∧
+                              (y4 = 0 ∨ 1 - y4 = 0)) ∧
+                            (y5 = 0 ∨ 1 - y5 = 0)) ∧
+                          (y6 = 0 ∨ 1 - y6 = 0)) ∧
+                        (y7 = 0 ∨ 1 - y7 = 0)) ∧
+                      (y8 = 0 ∨ 1 - y8 = 0)))[props][{ name := "%116" }] ←
+                  ((((((((((y1 + y2 * 2 + y3 * 3 + y4 * 4 + y5 * 5 + y6 * 6 + y7 * 7 + y8 * 8 + y9 * 9 + y10 * 10 +
+                                                            y11 * 11 +
+                                                          y12 * 12 +
+                                                        y13 * 13 +
+                                                      y14 * 14 +
+                                                    y15 * 15 +
+                                                  y16 * 16 +
+                                                y17 * 17 +
+                                              y18 * 18 +
+                                            y19 * 19 -
+                                          x0 =
+                                        0 ∧
+                                      (y0 = 0 ∨ 1 - y0 = 0)) ∧
+                                    (y1 = 0 ∨ 1 - y1 = 0)) ∧
+                                  (y2 = 0 ∨ 1 - y2 = 0)) ∧
+                                (y3 = 0 ∨ 1 - y3 = 0)) ∧
+                              (y4 = 0 ∨ 1 - y4 = 0)) ∧
+                            (y5 = 0 ∨ 1 - y5 = 0)) ∧
+                          (y6 = 0 ∨ 1 - y6 = 0)) ∧
+                        (y7 = 0 ∨ 1 - y7 = 0)) ∧
+                      (y8 = 0 ∨ 1 - y8 = 0)) ∧
+                    (y9 = 0 ∨ 1 - y9 = 0)))[props][{ name := "%120" }] ←
+                (((((((((((y1 + y2 * 2 + y3 * 3 + y4 * 4 + y5 * 5 + y6 * 6 + y7 * 7 + y8 * 8 + y9 * 9 + y10 * 10 +
+                                                            y11 * 11 +
+                                                          y12 * 12 +
+                                                        y13 * 13 +
+                                                      y14 * 14 +
+                                                    y15 * 15 +
+                                                  y16 * 16 +
+                                                y17 * 17 +
+                                              y18 * 18 +
+                                            y19 * 19 -
+                                          x0 =
+                                        0 ∧
+                                      (y0 = 0 ∨ 1 - y0 = 0)) ∧
+                                    (y1 = 0 ∨ 1 - y1 = 0)) ∧
+                                  (y2 = 0 ∨ 1 - y2 = 0)) ∧
+                                (y3 = 0 ∨ 1 - y3 = 0)) ∧
+                              (y4 = 0 ∨ 1 - y4 = 0)) ∧
+                            (y5 = 0 ∨ 1 - y5 = 0)) ∧
+                          (y6 = 0 ∨ 1 - y6 = 0)) ∧
+                        (y7 = 0 ∨ 1 - y7 = 0)) ∧
+                      (y8 = 0 ∨ 1 - y8 = 0)) ∧
+                    (y9 = 0 ∨ 1 - y9 = 0)) ∧
+                  (y10 = 0 ∨ 1 - y10 = 0)))[props][{ name := "%124" }] ←
+              ((((((((((((y1 + y2 * 2 + y3 * 3 + y4 * 4 + y5 * 5 + y6 * 6 + y7 * 7 + y8 * 8 + y9 * 9 + y10 * 10 +
+                                                            y11 * 11 +
+                                                          y12 * 12 +
+                                                        y13 * 13 +
+                                                      y14 * 14 +
+                                                    y15 * 15 +
+                                                  y16 * 16 +
+                                                y17 * 17 +
+                                              y18 * 18 +
+                                            y19 * 19 -
+                                          x0 =
+                                        0 ∧
+                                      (y0 = 0 ∨ 1 - y0 = 0)) ∧
+                                    (y1 = 0 ∨ 1 - y1 = 0)) ∧
+                                  (y2 = 0 ∨ 1 - y2 = 0)) ∧
+                                (y3 = 0 ∨ 1 - y3 = 0)) ∧
+                              (y4 = 0 ∨ 1 - y4 = 0)) ∧
+                            (y5 = 0 ∨ 1 - y5 = 0)) ∧
+                          (y6 = 0 ∨ 1 - y6 = 0)) ∧
+                        (y7 = 0 ∨ 1 - y7 = 0)) ∧
+                      (y8 = 0 ∨ 1 - y8 = 0)) ∧
+                    (y9 = 0 ∨ 1 - y9 = 0)) ∧
+                  (y10 = 0 ∨ 1 - y10 = 0)) ∧
+                (y11 = 0 ∨ 1 - y11 = 0)))[felts][{ name := "%125" }] ←
+            y0 + y1 + y2 + y3 + y4 + y5 + y6 + y7 + y8 + y9 + y10 + y11)[felts][{ name := "%127" }] ←
+          y12 * (1 - y12)))  := by
+    rewrite [part31_cumulative_wp]
+    rewrite [part32_updates_opaque]
+    unfold part31_state
+    MLIR_states_updates
+    -- 0 withEqZeros
+    -- rewrite [withEqZero_def]
+    -- MLIR_states_updates
+    unfold part31_drops
+    -- 4 drops
+    simp only [State.drop_update_swap, State.drop_update_same, State.drop_updateProps_swap]
+    rewrite [State.dropFelts]
+    simp only [State.dropFelts_buffers, State.dropFelts_bufferWidths, State.dropFelts_constraints, State.dropFelts_cycle, State.dropFelts_felts, State.dropFelts_isFailed, State.dropFelts_props, State.dropFelts_vars]
+    simp only [Map.drop_base, ne_eq, Map.update_drop_swap, Map.update_drop]
+    -- 0 sets
+    -- rewrite [Map.drop_of_updates]
+    -- simp only [Map.drop_base, ne_eq, Map.update_drop_swap, Map.update_drop]
 
 end Risc0.OneHot20.Constraints.WP
