Risc0/Gadgets/OneHot20/Constraints/WeakestPresPart39.lean
@@ -8,33 +8,600 @@ namespace Risc0.OneHot20.Constraints.WP
 open MLIRNotation
 
 -- The state obtained by running Code.part39 on st
-def part39_state (st: State) : State := 
+def part39_state (st: State) : State :=
   
-      ((((st[props][{ name := "%156" }] ←
-              (Option.get! (State.props st { name := "%152" }) ∧
-                Option.get! (State.felts st { name := "%155" }) = 0))[felts][{ name := "%157" }] ←
-            Option.get! (State.felts st { name := "%153" }) +
-              Option.get! (State.felts st { name := "%73" }))[felts][{ name := "%158" }] ←
-          Option.get! (State.felts st { name := "%153" }) + Option.get! (State.felts st { name := "%73" }) -
-            Option.get! (State.felts st { name := "%0" }))[props][{ name := "%159" }] ←
-        ((Option.get! (State.props st { name := "%152" }) ∧ Option.get! (State.felts st { name := "%155" }) = 0) ∧
-          Option.get! (State.felts st { name := "%153" }) + Option.get! (State.felts st { name := "%73" }) -
-              Option.get! (State.felts st { name := "%0" }) =
-            0)) 
+        ((((st[props][{ name := "%156" }] ←
+                (Option.get! (State.props st { name := "%152" }) ∧
+                  Option.get! (State.felts st { name := "%155" }) = 0))[felts][{ name := "%157" }] ←
+              Option.get! (State.felts st { name := "%153" }) +
+                Option.get! (State.felts st { name := "%73" }))[felts][{ name := "%158" }] ←
+            Option.get! (State.felts st { name := "%153" }) + Option.get! (State.felts st { name := "%73" }) -
+              Option.get! (State.felts st { name := "%0" }))[props][{ name := "%159" }] ←
+          ((Option.get! (State.props st { name := "%152" }) ∧ Option.get! (State.felts st { name := "%155" }) = 0) ∧
+            Option.get! (State.felts st { name := "%153" }) + Option.get! (State.felts st { name := "%73" }) -
+                Option.get! (State.felts st { name := "%0" }) =
+              0)) 
+
+def part39_drops (st: State) : State :=
+  State.dropFelts (State.dropFelts (State.dropFelts (State.dropFelts (State.dropFelts (State.dropFelts (State.dropFelts (State.dropFelts (State.dropFelts (State.dropFelts (State.dropFelts (State.dropFelts (State.dropFelts (State.dropFelts (State.dropFelts (State.dropFelts (State.dropFelts (State.dropFelts (State.dropFelts (State.dropFelts (State.dropFelts (State.dropFelts (State.dropFelts (State.dropFelts (State.dropFelts (State.dropFelts (State.dropFelts (State.dropFelts (State.dropFelts (st) ⟨"%19"⟩) ⟨"%73"⟩) ⟨"%77"⟩) ⟨"%0"⟩) ⟨"%81"⟩) ⟨"%84"⟩) ⟨"%88"⟩) ⟨"%92"⟩) ⟨"%96"⟩) ⟨"%100"⟩) ⟨"%104"⟩) ⟨"%108"⟩) ⟨"%112"⟩) ⟨"%116"⟩) ⟨"%120"⟩) ⟨"%124"⟩) ⟨"%128"⟩) ⟨"%132"⟩) ⟨"%136"⟩) ⟨"%140"⟩) ⟨"%144"⟩) ⟨"%148"⟩) ⟨"%152"⟩) ⟨"%153"⟩) ⟨"%155"⟩) ⟨"%156"⟩) ⟨"%157"⟩) ⟨"%158"⟩) ⟨"%159"⟩
+
+-- Run the program from part39 onwards by using part39_state rather than Code.part39
+def part39_state_update (st: State): State :=
+  part39_drops (part39_state st)
 
 -- Prove that substituting part39_state for Code.part39 produces the same result
-lemma part39_wp {st : State} :
-  Code.getReturn (MLIR.runProgram Code.part39 st) ↔
-  Code.getReturn (part39_state st) := by
+lemma part39_wp {st : State}:
+  Code.getReturn (MLIR.runProgram (Code.part39;dropfelt ⟨"%19"⟩;dropfelt ⟨"%73"⟩;dropfelt ⟨"%77"⟩;dropfelt ⟨"%0"⟩;dropfelt ⟨"%81"⟩;dropfelt ⟨"%84"⟩;dropfelt ⟨"%88"⟩;dropfelt ⟨"%92"⟩;dropfelt ⟨"%96"⟩;dropfelt ⟨"%100"⟩;dropfelt ⟨"%104"⟩;dropfelt ⟨"%108"⟩;dropfelt ⟨"%112"⟩;dropfelt ⟨"%116"⟩;dropfelt ⟨"%120"⟩;dropfelt ⟨"%124"⟩;dropfelt ⟨"%128"⟩;dropfelt ⟨"%132"⟩;dropfelt ⟨"%136"⟩;dropfelt ⟨"%140"⟩;dropfelt ⟨"%144"⟩;dropfelt ⟨"%148"⟩;dropfelt ⟨"%152"⟩;dropfelt ⟨"%153"⟩;dropfelt ⟨"%155"⟩;dropfelt ⟨"%156"⟩;dropfelt ⟨"%157"⟩;dropfelt ⟨"%158"⟩;dropfelt ⟨"%159"⟩) st) ↔
+  Code.getReturn (part39_state_update st) := by
   unfold MLIR.runProgram; simp only
+  generalize eq : (dropfelt ⟨"%19"⟩;dropfelt ⟨"%73"⟩;dropfelt ⟨"%77"⟩;dropfelt ⟨"%0"⟩;dropfelt ⟨"%81"⟩;dropfelt ⟨"%84"⟩;dropfelt ⟨"%88"⟩;dropfelt ⟨"%92"⟩;dropfelt ⟨"%96"⟩;dropfelt ⟨"%100"⟩;dropfelt ⟨"%104"⟩;dropfelt ⟨"%108"⟩;dropfelt ⟨"%112"⟩;dropfelt ⟨"%116"⟩;dropfelt ⟨"%120"⟩;dropfelt ⟨"%124"⟩;dropfelt ⟨"%128"⟩;dropfelt ⟨"%132"⟩;dropfelt ⟨"%136"⟩;dropfelt ⟨"%140"⟩;dropfelt ⟨"%144"⟩;dropfelt ⟨"%148"⟩;dropfelt ⟨"%152"⟩;dropfelt ⟨"%153"⟩;dropfelt ⟨"%155"⟩;dropfelt ⟨"%156"⟩;dropfelt ⟨"%157"⟩;dropfelt ⟨"%158"⟩;dropfelt ⟨"%159"⟩) = prog
   unfold Code.part39
   MLIR
-  unfold part39_state
+  rewrite [←eq]
+  rewrite [MLIR.run_seq_def,MLIR.run_dropfelt, MLIR.run_seq_def,MLIR.run_dropfelt, MLIR.run_seq_def,MLIR.run_dropfelt, MLIR.run_seq_def,MLIR.run_dropfelt, MLIR.run_seq_def,MLIR.run_dropfelt, MLIR.run_seq_def,MLIR.run_dropfelt, MLIR.run_seq_def,MLIR.run_dropfelt, MLIR.run_seq_def,MLIR.run_dropfelt, MLIR.run_seq_def,MLIR.run_dropfelt, MLIR.run_seq_def,MLIR.run_dropfelt, MLIR.run_seq_def,MLIR.run_dropfelt, MLIR.run_seq_def,MLIR.run_dropfelt, MLIR.run_seq_def,MLIR.run_dropfelt, MLIR.run_seq_def,MLIR.run_dropfelt, MLIR.run_seq_def,MLIR.run_dropfelt, MLIR.run_seq_def,MLIR.run_dropfelt, MLIR.run_seq_def,MLIR.run_dropfelt, MLIR.run_seq_def,MLIR.run_dropfelt, MLIR.run_seq_def,MLIR.run_dropfelt, MLIR.run_seq_def,MLIR.run_dropfelt, MLIR.run_seq_def,MLIR.run_dropfelt, MLIR.run_seq_def,MLIR.run_dropfelt, MLIR.run_seq_def,MLIR.run_dropfelt, MLIR.run_seq_def,MLIR.run_dropfelt, MLIR.run_seq_def,MLIR.run_dropfelt, MLIR.run_seq_def,MLIR.run_dropfelt, MLIR.run_seq_def,MLIR.run_dropfelt, MLIR.run_seq_def,MLIR.run_dropfelt, MLIR.run_dropfelt]
+  unfold part39_state_update part39_drops part39_state
   rfl
 
 lemma part39_updates_opaque {st : State} : 
   Code.getReturn (part38_state_update st) ↔
-  Code.getReturn (part39_state (part38_state st)) := by
+  Code.getReturn (part39_state_update (part38_drops (part38_state st))) := by
   simp [part38_state_update, part39_wp]
 
+lemma part39_cumulative_wp {x0 y0 y1 y2 y3 y4 y5 y6 y7 y8 y9 y10 y11 y12 y13 y14 y15 y16 y17 y18 y19: Felt} :
+  Code.run (start_state [x0] ([y0,y1,y2,y3,y4,y5,y6,y7,y8,y9,y10,y11,y12,y13,y14,y15,y16,y17,y18,y19])) ↔
+  Code.getReturn
+      (part39_state_update
+        ((((((((((((((((((((((((({
+                                                            buffers :=
+                                                              ((fun x => Map.empty x)[{ name := "data" }] ←ₘ
+                                                                  [[some y0, some y1, some y2, some y3, some y4,
+                                                                      some y5, some y6, some y7, some y8, some y9,
+                                                                      some y10, some y11, some y12, some y13, some y14,
+                                                                      some y15, some y16, some y17, some y18,
+                                                                      some y19]])[{ name := "code" }] ←ₘ
+                                                                [[some x0]],
+                                                            bufferWidths :=
+                                                              ((fun x => Map.empty x)[{ name := "data" }] ←ₘ
+                                                                  20)[{ name := "code" }] ←ₘ
+                                                                1,
+                                                            constraints := [], cycle := 0, felts := Map.empty,
+                                                            isFailed := false, props := Map.empty,
+                                                            vars :=
+                                                              [{ name := "code" },
+                                                                { name := "data" }] }[props][{ name := "%19" }] ←
+                                                          True)[felts][{ name := "%73" }] ←
+                                                        y19)[props][{ name := "%77" }] ←
+                                                      y1 + y2 * 2 + y3 * 3 + y4 * 4 + y5 * 5 + y6 * 6 + y7 * 7 +
+                                                                                  y8 * 8 +
+                                                                                y9 * 9 +
+                                                                              y10 * 10 +
+                                                                            y11 * 11 +
+                                                                          y12 * 12 +
+                                                                        y13 * 13 +
+                                                                      y14 * 14 +
+                                                                    y15 * 15 +
+                                                                  y16 * 16 +
+                                                                y17 * 17 +
+                                                              y18 * 18 +
+                                                            y19 * 19 -
+                                                          x0 =
+                                                        0)[felts][{ name := "%0" }] ←
+                                                    1)[props][{ name := "%81" }] ←
+                                                  (y1 + y2 * 2 + y3 * 3 + y4 * 4 + y5 * 5 + y6 * 6 + y7 * 7 + y8 * 8 +
+                                                                              y9 * 9 +
+                                                                            y10 * 10 +
+                                                                          y11 * 11 +
+                                                                        y12 * 12 +
+                                                                      y13 * 13 +
+                                                                    y14 * 14 +
+                                                                  y15 * 15 +
+                                                                y16 * 16 +
+                                                              y17 * 17 +
+                                                            y18 * 18 +
+                                                          y19 * 19 -
+                                                        x0 =
+                                                      0 ∧
+                                                    (y0 = 0 ∨ 1 - y0 = 0)))[props][{ name := "%84" }] ←
+                                                ((y1 + y2 * 2 + y3 * 3 + y4 * 4 + y5 * 5 + y6 * 6 + y7 * 7 + y8 * 8 +
+                                                                              y9 * 9 +
+                                                                            y10 * 10 +
+                                                                          y11 * 11 +
+                                                                        y12 * 12 +
+                                                                      y13 * 13 +
+                                                                    y14 * 14 +
+                                                                  y15 * 15 +
+                                                                y16 * 16 +
+                                                              y17 * 17 +
+                                                            y18 * 18 +
+                                                          y19 * 19 -
+                                                        x0 =
+                                                      0 ∧
+                                                    (y0 = 0 ∨ 1 - y0 = 0)) ∧
+                                                  (y1 = 0 ∨ 1 - y1 = 0)))[props][{ name := "%88" }] ←
+                                              (((y1 + y2 * 2 + y3 * 3 + y4 * 4 + y5 * 5 + y6 * 6 + y7 * 7 + y8 * 8 +
+                                                                              y9 * 9 +
+                                                                            y10 * 10 +
+                                                                          y11 * 11 +
+                                                                        y12 * 12 +
+                                                                      y13 * 13 +
+                                                                    y14 * 14 +
+                                                                  y15 * 15 +
+                                                                y16 * 16 +
+                                                              y17 * 17 +
+                                                            y18 * 18 +
+                                                          y19 * 19 -
+                                                        x0 =
+                                                      0 ∧
+                                                    (y0 = 0 ∨ 1 - y0 = 0)) ∧
+                                                  (y1 = 0 ∨ 1 - y1 = 0)) ∧
+                                                (y2 = 0 ∨ 1 - y2 = 0)))[props][{ name := "%92" }] ←
+                                            ((((y1 + y2 * 2 + y3 * 3 + y4 * 4 + y5 * 5 + y6 * 6 + y7 * 7 + y8 * 8 +
+                                                                              y9 * 9 +
+                                                                            y10 * 10 +
+                                                                          y11 * 11 +
+                                                                        y12 * 12 +
+                                                                      y13 * 13 +
+                                                                    y14 * 14 +
+                                                                  y15 * 15 +
+                                                                y16 * 16 +
+                                                              y17 * 17 +
+                                                            y18 * 18 +
+                                                          y19 * 19 -
+                                                        x0 =
+                                                      0 ∧
+                                                    (y0 = 0 ∨ 1 - y0 = 0)) ∧
+                                                  (y1 = 0 ∨ 1 - y1 = 0)) ∧
+                                                (y2 = 0 ∨ 1 - y2 = 0)) ∧
+                                              (y3 = 0 ∨ 1 - y3 = 0)))[props][{ name := "%96" }] ←
+                                          (((((y1 + y2 * 2 + y3 * 3 + y4 * 4 + y5 * 5 + y6 * 6 + y7 * 7 + y8 * 8 +
+                                                                              y9 * 9 +
+                                                                            y10 * 10 +
+                                                                          y11 * 11 +
+                                                                        y12 * 12 +
+                                                                      y13 * 13 +
+                                                                    y14 * 14 +
+                                                                  y15 * 15 +
+                                                                y16 * 16 +
+                                                              y17 * 17 +
+                                                            y18 * 18 +
+                                                          y19 * 19 -
+                                                        x0 =
+                                                      0 ∧
+                                                    (y0 = 0 ∨ 1 - y0 = 0)) ∧
+                                                  (y1 = 0 ∨ 1 - y1 = 0)) ∧
+                                                (y2 = 0 ∨ 1 - y2 = 0)) ∧
+                                              (y3 = 0 ∨ 1 - y3 = 0)) ∧
+                                            (y4 = 0 ∨ 1 - y4 = 0)))[props][{ name := "%100" }] ←
+                                        ((((((y1 + y2 * 2 + y3 * 3 + y4 * 4 + y5 * 5 + y6 * 6 + y7 * 7 + y8 * 8 +
+                                                                              y9 * 9 +
+                                                                            y10 * 10 +
+                                                                          y11 * 11 +
+                                                                        y12 * 12 +
+                                                                      y13 * 13 +
+                                                                    y14 * 14 +
+                                                                  y15 * 15 +
+                                                                y16 * 16 +
+                                                              y17 * 17 +
+                                                            y18 * 18 +
+                                                          y19 * 19 -
+                                                        x0 =
+                                                      0 ∧
+                                                    (y0 = 0 ∨ 1 - y0 = 0)) ∧
+                                                  (y1 = 0 ∨ 1 - y1 = 0)) ∧
+                                                (y2 = 0 ∨ 1 - y2 = 0)) ∧
+                                              (y3 = 0 ∨ 1 - y3 = 0)) ∧
+                                            (y4 = 0 ∨ 1 - y4 = 0)) ∧
+                                          (y5 = 0 ∨ 1 - y5 = 0)))[props][{ name := "%104" }] ←
+                                      (((((((y1 + y2 * 2 + y3 * 3 + y4 * 4 + y5 * 5 + y6 * 6 + y7 * 7 + y8 * 8 +
+                                                                              y9 * 9 +
+                                                                            y10 * 10 +
+                                                                          y11 * 11 +
+                                                                        y12 * 12 +
+                                                                      y13 * 13 +
+                                                                    y14 * 14 +
+                                                                  y15 * 15 +
+                                                                y16 * 16 +
+                                                              y17 * 17 +
+                                                            y18 * 18 +
+                                                          y19 * 19 -
+                                                        x0 =
+                                                      0 ∧
+                                                    (y0 = 0 ∨ 1 - y0 = 0)) ∧
+                                                  (y1 = 0 ∨ 1 - y1 = 0)) ∧
+                                                (y2 = 0 ∨ 1 - y2 = 0)) ∧
+                                              (y3 = 0 ∨ 1 - y3 = 0)) ∧
+                                            (y4 = 0 ∨ 1 - y4 = 0)) ∧
+                                          (y5 = 0 ∨ 1 - y5 = 0)) ∧
+                                        (y6 = 0 ∨ 1 - y6 = 0)))[props][{ name := "%108" }] ←
+                                    ((((((((y1 + y2 * 2 + y3 * 3 + y4 * 4 + y5 * 5 + y6 * 6 + y7 * 7 + y8 * 8 + y9 * 9 +
+                                                                            y10 * 10 +
+                                                                          y11 * 11 +
+                                                                        y12 * 12 +
+                                                                      y13 * 13 +
+                                                                    y14 * 14 +
+                                                                  y15 * 15 +
+                                                                y16 * 16 +
+                                                              y17 * 17 +
+                                                            y18 * 18 +
+                                                          y19 * 19 -
+                                                        x0 =
+                                                      0 ∧
+                                                    (y0 = 0 ∨ 1 - y0 = 0)) ∧
+                                                  (y1 = 0 ∨ 1 - y1 = 0)) ∧
+                                                (y2 = 0 ∨ 1 - y2 = 0)) ∧
+                                              (y3 = 0 ∨ 1 - y3 = 0)) ∧
+                                            (y4 = 0 ∨ 1 - y4 = 0)) ∧
+                                          (y5 = 0 ∨ 1 - y5 = 0)) ∧
+                                        (y6 = 0 ∨ 1 - y6 = 0)) ∧
+                                      (y7 = 0 ∨ 1 - y7 = 0)))[props][{ name := "%112" }] ←
+                                  (((((((((y1 + y2 * 2 + y3 * 3 + y4 * 4 + y5 * 5 + y6 * 6 + y7 * 7 + y8 * 8 + y9 * 9 +
+                                                                            y10 * 10 +
+                                                                          y11 * 11 +
+                                                                        y12 * 12 +
+                                                                      y13 * 13 +
+                                                                    y14 * 14 +
+                                                                  y15 * 15 +
+                                                                y16 * 16 +
+                                                              y17 * 17 +
+                                                            y18 * 18 +
+                                                          y19 * 19 -
+                                                        x0 =
+                                                      0 ∧
+                                                    (y0 = 0 ∨ 1 - y0 = 0)) ∧
+                                                  (y1 = 0 ∨ 1 - y1 = 0)) ∧
+                                                (y2 = 0 ∨ 1 - y2 = 0)) ∧
+                                              (y3 = 0 ∨ 1 - y3 = 0)) ∧
+                                            (y4 = 0 ∨ 1 - y4 = 0)) ∧
+                                          (y5 = 0 ∨ 1 - y5 = 0)) ∧
+                                        (y6 = 0 ∨ 1 - y6 = 0)) ∧
+                                      (y7 = 0 ∨ 1 - y7 = 0)) ∧
+                                    (y8 = 0 ∨ 1 - y8 = 0)))[props][{ name := "%116" }] ←
+                                ((((((((((y1 + y2 * 2 + y3 * 3 + y4 * 4 + y5 * 5 + y6 * 6 + y7 * 7 + y8 * 8 + y9 * 9 +
+                                                                            y10 * 10 +
+                                                                          y11 * 11 +
+                                                                        y12 * 12 +
+                                                                      y13 * 13 +
+                                                                    y14 * 14 +
+                                                                  y15 * 15 +
+                                                                y16 * 16 +
+                                                              y17 * 17 +
+                                                            y18 * 18 +
+                                                          y19 * 19 -
+                                                        x0 =
+                                                      0 ∧
+                                                    (y0 = 0 ∨ 1 - y0 = 0)) ∧
+                                                  (y1 = 0 ∨ 1 - y1 = 0)) ∧
+                                                (y2 = 0 ∨ 1 - y2 = 0)) ∧
+                                              (y3 = 0 ∨ 1 - y3 = 0)) ∧
+                                            (y4 = 0 ∨ 1 - y4 = 0)) ∧
+                                          (y5 = 0 ∨ 1 - y5 = 0)) ∧
+                                        (y6 = 0 ∨ 1 - y6 = 0)) ∧
+                                      (y7 = 0 ∨ 1 - y7 = 0)) ∧
+                                    (y8 = 0 ∨ 1 - y8 = 0)) ∧
+                                  (y9 = 0 ∨ 1 - y9 = 0)))[props][{ name := "%120" }] ←
+                              (((((((((((y1 + y2 * 2 + y3 * 3 + y4 * 4 + y5 * 5 + y6 * 6 + y7 * 7 + y8 * 8 + y9 * 9 +
+                                                                            y10 * 10 +
+                                                                          y11 * 11 +
+                                                                        y12 * 12 +
+                                                                      y13 * 13 +
+                                                                    y14 * 14 +
+                                                                  y15 * 15 +
+                                                                y16 * 16 +
+                                                              y17 * 17 +
+                                                            y18 * 18 +
+                                                          y19 * 19 -
+                                                        x0 =
+                                                      0 ∧
+                                                    (y0 = 0 ∨ 1 - y0 = 0)) ∧
+                                                  (y1 = 0 ∨ 1 - y1 = 0)) ∧
+                                                (y2 = 0 ∨ 1 - y2 = 0)) ∧
+                                              (y3 = 0 ∨ 1 - y3 = 0)) ∧
+                                            (y4 = 0 ∨ 1 - y4 = 0)) ∧
+                                          (y5 = 0 ∨ 1 - y5 = 0)) ∧
+                                        (y6 = 0 ∨ 1 - y6 = 0)) ∧
+                                      (y7 = 0 ∨ 1 - y7 = 0)) ∧
+                                    (y8 = 0 ∨ 1 - y8 = 0)) ∧
+                                  (y9 = 0 ∨ 1 - y9 = 0)) ∧
+                                (y10 = 0 ∨ 1 - y10 = 0)))[props][{ name := "%124" }] ←
+                            ((((((((((((y1 + y2 * 2 + y3 * 3 + y4 * 4 + y5 * 5 + y6 * 6 + y7 * 7 + y8 * 8 + y9 * 9 +
+                                                                            y10 * 10 +
+                                                                          y11 * 11 +
+                                                                        y12 * 12 +
+                                                                      y13 * 13 +
+                                                                    y14 * 14 +
+                                                                  y15 * 15 +
+                                                                y16 * 16 +
+                                                              y17 * 17 +
+                                                            y18 * 18 +
+                                                          y19 * 19 -
+                                                        x0 =
+                                                      0 ∧
+                                                    (y0 = 0 ∨ 1 - y0 = 0)) ∧
+                                                  (y1 = 0 ∨ 1 - y1 = 0)) ∧
+                                                (y2 = 0 ∨ 1 - y2 = 0)) ∧
+                                              (y3 = 0 ∨ 1 - y3 = 0)) ∧
+                                            (y4 = 0 ∨ 1 - y4 = 0)) ∧
+                                          (y5 = 0 ∨ 1 - y5 = 0)) ∧
+                                        (y6 = 0 ∨ 1 - y6 = 0)) ∧
+                                      (y7 = 0 ∨ 1 - y7 = 0)) ∧
+                                    (y8 = 0 ∨ 1 - y8 = 0)) ∧
+                                  (y9 = 0 ∨ 1 - y9 = 0)) ∧
+                                (y10 = 0 ∨ 1 - y10 = 0)) ∧
+                              (y11 = 0 ∨ 1 - y11 = 0)))[props][{ name := "%128" }] ←
+                          (((((((((((((y1 + y2 * 2 + y3 * 3 + y4 * 4 + y5 * 5 + y6 * 6 + y7 * 7 + y8 * 8 + y9 * 9 +
+                                                                            y10 * 10 +
+                                                                          y11 * 11 +
+                                                                        y12 * 12 +
+                                                                      y13 * 13 +
+                                                                    y14 * 14 +
+                                                                  y15 * 15 +
+                                                                y16 * 16 +
+                                                              y17 * 17 +
+                                                            y18 * 18 +
+                                                          y19 * 19 -
+                                                        x0 =
+                                                      0 ∧
+                                                    (y0 = 0 ∨ 1 - y0 = 0)) ∧
+                                                  (y1 = 0 ∨ 1 - y1 = 0)) ∧
+                                                (y2 = 0 ∨ 1 - y2 = 0)) ∧
+                                              (y3 = 0 ∨ 1 - y3 = 0)) ∧
+                                            (y4 = 0 ∨ 1 - y4 = 0)) ∧
+                                          (y5 = 0 ∨ 1 - y5 = 0)) ∧
+                                        (y6 = 0 ∨ 1 - y6 = 0)) ∧
+                                      (y7 = 0 ∨ 1 - y7 = 0)) ∧
+                                    (y8 = 0 ∨ 1 - y8 = 0)) ∧
+                                  (y9 = 0 ∨ 1 - y9 = 0)) ∧
+                                (y10 = 0 ∨ 1 - y10 = 0)) ∧
+                              (y11 = 0 ∨ 1 - y11 = 0)) ∧
+                            (y12 = 0 ∨ 1 - y12 = 0)))[props][{ name := "%132" }] ←
+                        ((((((((((((((y1 + y2 * 2 + y3 * 3 + y4 * 4 + y5 * 5 + y6 * 6 + y7 * 7 + y8 * 8 + y9 * 9 +
+                                                                            y10 * 10 +
+                                                                          y11 * 11 +
+                                                                        y12 * 12 +
+                                                                      y13 * 13 +
+                                                                    y14 * 14 +
+                                                                  y15 * 15 +
+                                                                y16 * 16 +
+                                                              y17 * 17 +
+                                                            y18 * 18 +
+                                                          y19 * 19 -
+                                                        x0 =
+                                                      0 ∧
+                                                    (y0 = 0 ∨ 1 - y0 = 0)) ∧
+                                                  (y1 = 0 ∨ 1 - y1 = 0)) ∧
+                                                (y2 = 0 ∨ 1 - y2 = 0)) ∧
+                                              (y3 = 0 ∨ 1 - y3 = 0)) ∧
+                                            (y4 = 0 ∨ 1 - y4 = 0)) ∧
+                                          (y5 = 0 ∨ 1 - y5 = 0)) ∧
+                                        (y6 = 0 ∨ 1 - y6 = 0)) ∧
+                                      (y7 = 0 ∨ 1 - y7 = 0)) ∧
+                                    (y8 = 0 ∨ 1 - y8 = 0)) ∧
+                                  (y9 = 0 ∨ 1 - y9 = 0)) ∧
+                                (y10 = 0 ∨ 1 - y10 = 0)) ∧
+                              (y11 = 0 ∨ 1 - y11 = 0)) ∧
+                            (y12 = 0 ∨ 1 - y12 = 0)) ∧
+                          (y13 = 0 ∨ 1 - y13 = 0)))[props][{ name := "%136" }] ←
+                      (((((((((((((((y1 + y2 * 2 + y3 * 3 + y4 * 4 + y5 * 5 + y6 * 6 + y7 * 7 + y8 * 8 + y9 * 9 +
+                                                                            y10 * 10 +
+                                                                          y11 * 11 +
+                                                                        y12 * 12 +
+                                                                      y13 * 13 +
+                                                                    y14 * 14 +
+                                                                  y15 * 15 +
+                                                                y16 * 16 +
+                                                              y17 * 17 +
+                                                            y18 * 18 +
+                                                          y19 * 19 -
+                                                        x0 =
+                                                      0 ∧
+                                                    (y0 = 0 ∨ 1 - y0 = 0)) ∧
+                                                  (y1 = 0 ∨ 1 - y1 = 0)) ∧
+                                                (y2 = 0 ∨ 1 - y2 = 0)) ∧
+                                              (y3 = 0 ∨ 1 - y3 = 0)) ∧
+                                            (y4 = 0 ∨ 1 - y4 = 0)) ∧
+                                          (y5 = 0 ∨ 1 - y5 = 0)) ∧
+                                        (y6 = 0 ∨ 1 - y6 = 0)) ∧
+                                      (y7 = 0 ∨ 1 - y7 = 0)) ∧
+                                    (y8 = 0 ∨ 1 - y8 = 0)) ∧
+                                  (y9 = 0 ∨ 1 - y9 = 0)) ∧
+                                (y10 = 0 ∨ 1 - y10 = 0)) ∧
+                              (y11 = 0 ∨ 1 - y11 = 0)) ∧
+                            (y12 = 0 ∨ 1 - y12 = 0)) ∧
+                          (y13 = 0 ∨ 1 - y13 = 0)) ∧
+                        (y14 = 0 ∨ 1 - y14 = 0)))[props][{ name := "%140" }] ←
+                    ((((((((((((((((y1 + y2 * 2 + y3 * 3 + y4 * 4 + y5 * 5 + y6 * 6 + y7 * 7 + y8 * 8 + y9 * 9 +
+                                                                            y10 * 10 +
+                                                                          y11 * 11 +
+                                                                        y12 * 12 +
+                                                                      y13 * 13 +
+                                                                    y14 * 14 +
+                                                                  y15 * 15 +
+                                                                y16 * 16 +
+                                                              y17 * 17 +
+                                                            y18 * 18 +
+                                                          y19 * 19 -
+                                                        x0 =
+                                                      0 ∧
+                                                    (y0 = 0 ∨ 1 - y0 = 0)) ∧
+                                                  (y1 = 0 ∨ 1 - y1 = 0)) ∧
+                                                (y2 = 0 ∨ 1 - y2 = 0)) ∧
+                                              (y3 = 0 ∨ 1 - y3 = 0)) ∧
+                                            (y4 = 0 ∨ 1 - y4 = 0)) ∧
+                                          (y5 = 0 ∨ 1 - y5 = 0)) ∧
+                                        (y6 = 0 ∨ 1 - y6 = 0)) ∧
+                                      (y7 = 0 ∨ 1 - y7 = 0)) ∧
+                                    (y8 = 0 ∨ 1 - y8 = 0)) ∧
+                                  (y9 = 0 ∨ 1 - y9 = 0)) ∧
+                                (y10 = 0 ∨ 1 - y10 = 0)) ∧
+                              (y11 = 0 ∨ 1 - y11 = 0)) ∧
+                            (y12 = 0 ∨ 1 - y12 = 0)) ∧
+                          (y13 = 0 ∨ 1 - y13 = 0)) ∧
+                        (y14 = 0 ∨ 1 - y14 = 0)) ∧
+                      (y15 = 0 ∨ 1 - y15 = 0)))[props][{ name := "%144" }] ←
+                  (((((((((((((((((y1 + y2 * 2 + y3 * 3 + y4 * 4 + y5 * 5 + y6 * 6 + y7 * 7 + y8 * 8 + y9 * 9 +
+                                                                            y10 * 10 +
+                                                                          y11 * 11 +
+                                                                        y12 * 12 +
+                                                                      y13 * 13 +
+                                                                    y14 * 14 +
+                                                                  y15 * 15 +
+                                                                y16 * 16 +
+                                                              y17 * 17 +
+                                                            y18 * 18 +
+                                                          y19 * 19 -
+                                                        x0 =
+                                                      0 ∧
+                                                    (y0 = 0 ∨ 1 - y0 = 0)) ∧
+                                                  (y1 = 0 ∨ 1 - y1 = 0)) ∧
+                                                (y2 = 0 ∨ 1 - y2 = 0)) ∧
+                                              (y3 = 0 ∨ 1 - y3 = 0)) ∧
+                                            (y4 = 0 ∨ 1 - y4 = 0)) ∧
+                                          (y5 = 0 ∨ 1 - y5 = 0)) ∧
+                                        (y6 = 0 ∨ 1 - y6 = 0)) ∧
+                                      (y7 = 0 ∨ 1 - y7 = 0)) ∧
+                                    (y8 = 0 ∨ 1 - y8 = 0)) ∧
+                                  (y9 = 0 ∨ 1 - y9 = 0)) ∧
+                                (y10 = 0 ∨ 1 - y10 = 0)) ∧
+                              (y11 = 0 ∨ 1 - y11 = 0)) ∧
+                            (y12 = 0 ∨ 1 - y12 = 0)) ∧
+                          (y13 = 0 ∨ 1 - y13 = 0)) ∧
+                        (y14 = 0 ∨ 1 - y14 = 0)) ∧
+                      (y15 = 0 ∨ 1 - y15 = 0)) ∧
+                    (y16 = 0 ∨ 1 - y16 = 0)))[props][{ name := "%148" }] ←
+                ((((((((((((((((((y1 + y2 * 2 + y3 * 3 + y4 * 4 + y5 * 5 + y6 * 6 + y7 * 7 + y8 * 8 + y9 * 9 +
+                                                                            y10 * 10 +
+                                                                          y11 * 11 +
+                                                                        y12 * 12 +
+                                                                      y13 * 13 +
+                                                                    y14 * 14 +
+                                                                  y15 * 15 +
+                                                                y16 * 16 +
+                                                              y17 * 17 +
+                                                            y18 * 18 +
+                                                          y19 * 19 -
+                                                        x0 =
+                                                      0 ∧
+                                                    (y0 = 0 ∨ 1 - y0 = 0)) ∧
+                                                  (y1 = 0 ∨ 1 - y1 = 0)) ∧
+                                                (y2 = 0 ∨ 1 - y2 = 0)) ∧
+                                              (y3 = 0 ∨ 1 - y3 = 0)) ∧
+                                            (y4 = 0 ∨ 1 - y4 = 0)) ∧
+                                          (y5 = 0 ∨ 1 - y5 = 0)) ∧
+                                        (y6 = 0 ∨ 1 - y6 = 0)) ∧
+                                      (y7 = 0 ∨ 1 - y7 = 0)) ∧
+                                    (y8 = 0 ∨ 1 - y8 = 0)) ∧
+                                  (y9 = 0 ∨ 1 - y9 = 0)) ∧
+                                (y10 = 0 ∨ 1 - y10 = 0)) ∧
+                              (y11 = 0 ∨ 1 - y11 = 0)) ∧
+                            (y12 = 0 ∨ 1 - y12 = 0)) ∧
+                          (y13 = 0 ∨ 1 - y13 = 0)) ∧
+                        (y14 = 0 ∨ 1 - y14 = 0)) ∧
+                      (y15 = 0 ∨ 1 - y15 = 0)) ∧
+                    (y16 = 0 ∨ 1 - y16 = 0)) ∧
+                  (y17 = 0 ∨ 1 - y17 = 0)))[props][{ name := "%152" }] ←
+              (((((((((((((((((((y1 + y2 * 2 + y3 * 3 + y4 * 4 + y5 * 5 + y6 * 6 + y7 * 7 + y8 * 8 + y9 * 9 + y10 * 10 +
+                                                                          y11 * 11 +
+                                                                        y12 * 12 +
+                                                                      y13 * 13 +
+                                                                    y14 * 14 +
+                                                                  y15 * 15 +
+                                                                y16 * 16 +
+                                                              y17 * 17 +
+                                                            y18 * 18 +
+                                                          y19 * 19 -
+                                                        x0 =
+                                                      0 ∧
+                                                    (y0 = 0 ∨ 1 - y0 = 0)) ∧
+                                                  (y1 = 0 ∨ 1 - y1 = 0)) ∧
+                                                (y2 = 0 ∨ 1 - y2 = 0)) ∧
+                                              (y3 = 0 ∨ 1 - y3 = 0)) ∧
+                                            (y4 = 0 ∨ 1 - y4 = 0)) ∧
+                                          (y5 = 0 ∨ 1 - y5 = 0)) ∧
+                                        (y6 = 0 ∨ 1 - y6 = 0)) ∧
+                                      (y7 = 0 ∨ 1 - y7 = 0)) ∧
+                                    (y8 = 0 ∨ 1 - y8 = 0)) ∧
+                                  (y9 = 0 ∨ 1 - y9 = 0)) ∧
+                                (y10 = 0 ∨ 1 - y10 = 0)) ∧
+                              (y11 = 0 ∨ 1 - y11 = 0)) ∧
+                            (y12 = 0 ∨ 1 - y12 = 0)) ∧
+                          (y13 = 0 ∨ 1 - y13 = 0)) ∧
+                        (y14 = 0 ∨ 1 - y14 = 0)) ∧
+                      (y15 = 0 ∨ 1 - y15 = 0)) ∧
+                    (y16 = 0 ∨ 1 - y16 = 0)) ∧
+                  (y17 = 0 ∨ 1 - y17 = 0)) ∧
+                (y18 = 0 ∨ 1 - y18 = 0)))[felts][{ name := "%153" }] ←
+            y0 + y1 + y2 + y3 + y4 + y5 + y6 + y7 + y8 + y9 + y10 + y11 + y12 + y13 + y14 + y15 + y16 + y17 +
+              y18)[felts][{ name := "%155" }] ←
+          y19 * (1 - y19)))  := by
+    rewrite [part38_cumulative_wp]
+    rewrite [part39_updates_opaque]
+    unfold part38_state
+    MLIR_states_updates
+    -- 0 withEqZeros
+    -- rewrite [withEqZero_def]
+    -- MLIR_states_updates
+    unfold part38_drops
+    -- 4 drops
+    simp only [State.drop_update_swap, State.drop_update_same, State.drop_updateProps_swap]
+    rewrite [State.dropFelts]
+    simp only [State.dropFelts_buffers, State.dropFelts_bufferWidths, State.dropFelts_constraints, State.dropFelts_cycle, State.dropFelts_felts, State.dropFelts_isFailed, State.dropFelts_props, State.dropFelts_vars]
+    simp only [Map.drop_base, ne_eq, Map.update_drop_swap, Map.update_drop]
+    -- 0 sets
+    -- rewrite [Map.drop_of_updates]
+    -- simp only [Map.drop_base, ne_eq, Map.update_drop_swap, Map.update_drop]
+
+lemma closed_form {x0 y0 y1 y2 y3 y4 y5 y6 y7 y8 y9 y10 y11 y12 y13 y14 y15 y16 y17 y18 y19: Felt} :
+  Code.run (start_state [x0] ([y0,y1,y2,y3,y4,y5,y6,y7,y8,y9,y10,y11,y12,y13,y14,y15,y16,y17,y18,y19])) ↔
+   ((((((((((((((((((((y1 + y2 * 2 + y3 * 3 + y4 * 4 + y5 * 5 + y6 * 6 + y7 * 7 + y8 * 8 + y9 * 9 + y10 * 10 + y11 * 11 +
+                                                                  y12 * 12 +
+                                                                y13 * 13 +
+                                                              y14 * 14 +
+                                                            y15 * 15 +
+                                                          y16 * 16 +
+                                                        y17 * 17 +
+                                                      y18 * 18 +
+                                                    y19 * 19 -
+                                                  x0 =
+                                                0 ∧
+                                              (y0 = 0 ∨ 1 - y0 = 0)) ∧
+                                            (y1 = 0 ∨ 1 - y1 = 0)) ∧
+                                          (y2 = 0 ∨ 1 - y2 = 0)) ∧
+                                        (y3 = 0 ∨ 1 - y3 = 0)) ∧
+                                      (y4 = 0 ∨ 1 - y4 = 0)) ∧
+                                    (y5 = 0 ∨ 1 - y5 = 0)) ∧
+                                  (y6 = 0 ∨ 1 - y6 = 0)) ∧
+                                (y7 = 0 ∨ 1 - y7 = 0)) ∧
+                              (y8 = 0 ∨ 1 - y8 = 0)) ∧
+                            (y9 = 0 ∨ 1 - y9 = 0)) ∧
+                          (y10 = 0 ∨ 1 - y10 = 0)) ∧
+                        (y11 = 0 ∨ 1 - y11 = 0)) ∧
+                      (y12 = 0 ∨ 1 - y12 = 0)) ∧
+                    (y13 = 0 ∨ 1 - y13 = 0)) ∧
+                  (y14 = 0 ∨ 1 - y14 = 0)) ∧
+                (y15 = 0 ∨ 1 - y15 = 0)) ∧
+              (y16 = 0 ∨ 1 - y16 = 0)) ∧
+            (y17 = 0 ∨ 1 - y17 = 0)) ∧
+          (y18 = 0 ∨ 1 - y18 = 0)) ∧
+        (y19 = 0 ∨ 1 - y19 = 0)) ∧
+      y0 + y1 + y2 + y3 + y4 + y5 + y6 + y7 + y8 + y9 + y10 + y11 + y12 + y13 + y14 + y15 + y16 + y17 + y18 + y19 - 1 =
+        0  := by
+    rewrite [part39_cumulative_wp]
+    unfold part39_state_update
+    unfold part39_state
+    MLIR_states_updates
+    -- 0 withEqZeros
+    -- rewrite [withEqZero_def]
+    -- MLIR_states_updates
+    unfold part39_drops
+    -- 29 drops
+    simp only [State.drop_update_swap, State.drop_update_same, State.drop_updateProps_swap]
+    rewrite [State.dropFelts]
+    simp only [State.dropFelts_buffers, State.dropFelts_bufferWidths, State.dropFelts_constraints, State.dropFelts_cycle, State.dropFelts_felts, State.dropFelts_isFailed, State.dropFelts_props, State.dropFelts_vars]
+    simp only [Map.drop_base, ne_eq, Map.update_drop_swap, Map.update_drop]
+    -- 0 sets
+    -- rewrite [Map.drop_of_updates]
+    -- simp only [Map.drop_base, ne_eq, Map.update_drop_swap, Map.update_drop]
+    unfold Code.getReturn
+    simp only
+    simp only [Code.getReturn, State.constraintsInVar, State.updateProps_props_get_wobbly, Option.getD_some]
 end Risc0.OneHot20.Constraints.WP
