Risc0/Gadgets/OneHot20/Witness/WeakestPresPart19.lean
@@ -9,10 +9,8 @@ open MLIRNotation
 
 -- The state obtained by running Code.part19 on st
 def part19_state (st: State) : State :=
-  
-          (State.set!
-            ((State.set! st { name := "data" } 18
-                  (Option.get! st.felts[({ name := "%174" }: FeltVar)]!)[felts][{ name := "%175" }] ←
+  ((State.set!
+            ((st[felts][{ name := "%175" }] ←
                 Option.get! (State.felts st { name := "%20" }) -
                   Option.get! (State.felts st { name := "%0" }))[felts][{ name := "%176" }] ←
               if Option.get! (State.felts st { name := "%20" }) - Option.get! (State.felts st { name := "%0" }) = 0 then
@@ -21,28 +19,98 @@ def part19_state (st: State) : State :=
             { name := "data" } 19
             (if Option.get! (State.felts st { name := "%20" }) - Option.get! (State.felts st { name := "%0" }) = 0 then
               1
-            else
-              0)) 
+            else 0))["%22"] ←ₛ
+          getImpl
+            ((st[felts][{ name := "%175" }] ←
+                Option.get! (State.felts st { name := "%20" }) -
+                  Option.get! (State.felts st { name := "%0" }))[felts][{ name := "%176" }] ←
+              if Option.get! (State.felts st { name := "%20" }) - Option.get! (State.felts st { name := "%0" }) = 0 then
+                1
+              else 0)
+            { name := "data" } 0 2)
+
+def part19_drops (st: State) : State :=
+  State.dropFelts (State.dropFelts (st) ⟨"%175"⟩) ⟨"%176"⟩
 
 -- Run the program from part19 onwards by using part19_state rather than Code.part19
 def part19_state_update (st: State): State :=
-  Γ (part19_state st) ⟦Code.part20; Code.part21; Code.part22; Code.part23; Code.part24; Code.part25; Code.part26; Code.part27; Code.part28; Code.part29; Code.part30; Code.part31; Code.part32; Code.part33; Code.part34; Code.part35; Code.part36; Code.part37; Code.part38; Code.part39; Code.part40; Code.part41; Code.part42; Code.part43; Code.part44; Code.part45; Code.part46; Code.part47; Code.part48; Code.part49; Code.part50; Code.part51; Code.part52; Code.part53; Code.part54⟧
+  Γ (part19_drops (part19_state st)) ⟦Code.part20;dropfelt ⟨"%17"⟩;dropfelt ⟨"%23"⟩;Code.part21;dropfelt ⟨"%16"⟩;dropfelt ⟨"%15"⟩;dropfelt ⟨"%24"⟩;dropfelt ⟨"%26"⟩;Code.part22;dropfelt ⟨"%14"⟩;dropfelt ⟨"%27"⟩;dropfelt ⟨"%29"⟩;dropfelt ⟨"%30"⟩;dropfelt ⟨"%32"⟩;Code.part23;dropfelt ⟨"%13"⟩;dropfelt ⟨"%33"⟩;dropfelt ⟨"%35"⟩;Code.part24;dropfelt ⟨"%12"⟩;dropfelt ⟨"%11"⟩;dropfelt ⟨"%36"⟩;dropfelt ⟨"%38"⟩;Code.part25;dropfelt ⟨"%10"⟩;dropfelt ⟨"%39"⟩;dropfelt ⟨"%41"⟩;dropfelt ⟨"%42"⟩;dropfelt ⟨"%44"⟩;Code.part26;dropfelt ⟨"%9"⟩;dropfelt ⟨"%45"⟩;dropfelt ⟨"%47"⟩;Code.part27;dropfelt ⟨"%8"⟩;dropfelt ⟨"%7"⟩;dropfelt ⟨"%48"⟩;dropfelt ⟨"%50"⟩;Code.part28;dropfelt ⟨"%6"⟩;dropfelt ⟨"%51"⟩;dropfelt ⟨"%53"⟩;dropfelt ⟨"%54"⟩;dropfelt ⟨"%56"⟩;Code.part29;dropfelt ⟨"%5"⟩;dropfelt ⟨"%57"⟩;dropfelt ⟨"%59"⟩;Code.part30;dropfelt ⟨"%4"⟩;dropfelt ⟨"%3"⟩;dropfelt ⟨"%60"⟩;dropfelt ⟨"%62"⟩;Code.part31;dropfelt ⟨"%2"⟩;dropfelt ⟨"%63"⟩;dropfelt ⟨"%65"⟩;dropfelt ⟨"%66"⟩;dropfelt ⟨"%68"⟩;Code.part32;dropfelt ⟨"%1"⟩;dropfelt ⟨"%69"⟩;dropfelt ⟨"%71"⟩;Code.part33;dropfelt ⟨"%20"⟩;dropfelt ⟨"%0"⟩;dropfelt ⟨"%72"⟩;dropfelt ⟨"%74"⟩;dropfelt ⟨"%75"⟩;dropfelt ⟨"%76"⟩;Code.part34;dropfelt ⟨"%78"⟩;dropfelt ⟨"%79"⟩;Code.part35;dropfelt ⟨"%21"⟩;dropfelt ⟨"%77"⟩;dropfelt ⟨"%80"⟩;dropfelt ⟨"%81"⟩;Code.part36;dropfelt ⟨"%22"⟩;dropfelt ⟨"%82"⟩;dropfelt ⟨"%83"⟩;dropfelt ⟨"%84"⟩;Code.part37;dropfelt ⟨"%25"⟩;dropfelt ⟨"%85"⟩;dropfelt ⟨"%86"⟩;dropfelt ⟨"%87"⟩;Code.part38;dropfelt ⟨"%28"⟩;dropfelt ⟨"%88"⟩;dropfelt ⟨"%89"⟩;dropfelt ⟨"%90"⟩;Code.part39;dropfelt ⟨"%31"⟩;dropfelt ⟨"%91"⟩;dropfelt ⟨"%92"⟩;dropfelt ⟨"%93"⟩;Code.part40;dropfelt ⟨"%34"⟩;dropfelt ⟨"%94"⟩;dropfelt ⟨"%95"⟩;dropfelt ⟨"%96"⟩;Code.part41;dropfelt ⟨"%37"⟩;dropfelt ⟨"%97"⟩;dropfelt ⟨"%98"⟩;dropfelt ⟨"%99"⟩;Code.part42;dropfelt ⟨"%40"⟩;dropfelt ⟨"%100"⟩;dropfelt ⟨"%101"⟩;dropfelt ⟨"%102"⟩;Code.part43;dropfelt ⟨"%43"⟩;dropfelt ⟨"%103"⟩;dropfelt ⟨"%104"⟩;dropfelt ⟨"%105"⟩;Code.part44;dropfelt ⟨"%46"⟩;dropfelt ⟨"%106"⟩;dropfelt ⟨"%107"⟩;dropfelt ⟨"%108"⟩;Code.part45;dropfelt ⟨"%49"⟩;dropfelt ⟨"%109"⟩;dropfelt ⟨"%110"⟩;dropfelt ⟨"%111"⟩;Code.part46;dropfelt ⟨"%52"⟩;dropfelt ⟨"%112"⟩;dropfelt ⟨"%113"⟩;dropfelt ⟨"%114"⟩;Code.part47;dropfelt ⟨"%55"⟩;dropfelt ⟨"%115"⟩;dropfelt ⟨"%116"⟩;dropfelt ⟨"%117"⟩;Code.part48;dropfelt ⟨"%58"⟩;dropfelt ⟨"%118"⟩;dropfelt ⟨"%119"⟩;dropfelt ⟨"%120"⟩;Code.part49;dropfelt ⟨"%61"⟩;dropfelt ⟨"%121"⟩;dropfelt ⟨"%122"⟩;dropfelt ⟨"%123"⟩;Code.part50;dropfelt ⟨"%64"⟩;dropfelt ⟨"%124"⟩;dropfelt ⟨"%125"⟩;dropfelt ⟨"%126"⟩;Code.part51;dropfelt ⟨"%67"⟩;dropfelt ⟨"%127"⟩;dropfelt ⟨"%128"⟩;dropfelt ⟨"%129"⟩;Code.part52;dropfelt ⟨"%70"⟩;dropfelt ⟨"%130"⟩;dropfelt ⟨"%131"⟩;dropfelt ⟨"%132"⟩;Code.part53;dropfelt ⟨"%73"⟩;dropfelt ⟨"%133"⟩;dropfelt ⟨"%134"⟩;dropfelt ⟨"%135"⟩;Code.part54;dropfelt ⟨"%18"⟩;dropfelt ⟨"%136"⟩;dropfelt ⟨"%137"⟩;dropfelt ⟨"%19"⟩⟧
 
 -- Prove that substituting part19_state for Code.part19 produces the same result
 lemma part19_wp {st : State} {y0 y1 y2 y3 y4 y5 y6 y7 y8 y9 y10 y11 y12 y13 y14 y15 y16 y17 y18 y19 : Option Felt} :
-  Code.getReturn (MLIR.runProgram (Code.part19; Code.part20; Code.part21; Code.part22; Code.part23; Code.part24; Code.part25; Code.part26; Code.part27; Code.part28; Code.part29; Code.part30; Code.part31; Code.part32; Code.part33; Code.part34; Code.part35; Code.part36; Code.part37; Code.part38; Code.part39; Code.part40; Code.part41; Code.part42; Code.part43; Code.part44; Code.part45; Code.part46; Code.part47; Code.part48; Code.part49; Code.part50; Code.part51; Code.part52; Code.part53; Code.part54) st) = [y0, y1, y2, y3, y4, y5, y6, y7, y8, y9, y10, y11, y12, y13, y14, y15, y16, y17, y18, y19] ↔
+  Code.getReturn (MLIR.runProgram (Code.part19;dropfelt ⟨"%175"⟩;dropfelt ⟨"%176"⟩;Code.part20;dropfelt ⟨"%17"⟩;dropfelt ⟨"%23"⟩;Code.part21;dropfelt ⟨"%16"⟩;dropfelt ⟨"%15"⟩;dropfelt ⟨"%24"⟩;dropfelt ⟨"%26"⟩;Code.part22;dropfelt ⟨"%14"⟩;dropfelt ⟨"%27"⟩;dropfelt ⟨"%29"⟩;dropfelt ⟨"%30"⟩;dropfelt ⟨"%32"⟩;Code.part23;dropfelt ⟨"%13"⟩;dropfelt ⟨"%33"⟩;dropfelt ⟨"%35"⟩;Code.part24;dropfelt ⟨"%12"⟩;dropfelt ⟨"%11"⟩;dropfelt ⟨"%36"⟩;dropfelt ⟨"%38"⟩;Code.part25;dropfelt ⟨"%10"⟩;dropfelt ⟨"%39"⟩;dropfelt ⟨"%41"⟩;dropfelt ⟨"%42"⟩;dropfelt ⟨"%44"⟩;Code.part26;dropfelt ⟨"%9"⟩;dropfelt ⟨"%45"⟩;dropfelt ⟨"%47"⟩;Code.part27;dropfelt ⟨"%8"⟩;dropfelt ⟨"%7"⟩;dropfelt ⟨"%48"⟩;dropfelt ⟨"%50"⟩;Code.part28;dropfelt ⟨"%6"⟩;dropfelt ⟨"%51"⟩;dropfelt ⟨"%53"⟩;dropfelt ⟨"%54"⟩;dropfelt ⟨"%56"⟩;Code.part29;dropfelt ⟨"%5"⟩;dropfelt ⟨"%57"⟩;dropfelt ⟨"%59"⟩;Code.part30;dropfelt ⟨"%4"⟩;dropfelt ⟨"%3"⟩;dropfelt ⟨"%60"⟩;dropfelt ⟨"%62"⟩;Code.part31;dropfelt ⟨"%2"⟩;dropfelt ⟨"%63"⟩;dropfelt ⟨"%65"⟩;dropfelt ⟨"%66"⟩;dropfelt ⟨"%68"⟩;Code.part32;dropfelt ⟨"%1"⟩;dropfelt ⟨"%69"⟩;dropfelt ⟨"%71"⟩;Code.part33;dropfelt ⟨"%20"⟩;dropfelt ⟨"%0"⟩;dropfelt ⟨"%72"⟩;dropfelt ⟨"%74"⟩;dropfelt ⟨"%75"⟩;dropfelt ⟨"%76"⟩;Code.part34;dropfelt ⟨"%78"⟩;dropfelt ⟨"%79"⟩;Code.part35;dropfelt ⟨"%21"⟩;dropfelt ⟨"%77"⟩;dropfelt ⟨"%80"⟩;dropfelt ⟨"%81"⟩;Code.part36;dropfelt ⟨"%22"⟩;dropfelt ⟨"%82"⟩;dropfelt ⟨"%83"⟩;dropfelt ⟨"%84"⟩;Code.part37;dropfelt ⟨"%25"⟩;dropfelt ⟨"%85"⟩;dropfelt ⟨"%86"⟩;dropfelt ⟨"%87"⟩;Code.part38;dropfelt ⟨"%28"⟩;dropfelt ⟨"%88"⟩;dropfelt ⟨"%89"⟩;dropfelt ⟨"%90"⟩;Code.part39;dropfelt ⟨"%31"⟩;dropfelt ⟨"%91"⟩;dropfelt ⟨"%92"⟩;dropfelt ⟨"%93"⟩;Code.part40;dropfelt ⟨"%34"⟩;dropfelt ⟨"%94"⟩;dropfelt ⟨"%95"⟩;dropfelt ⟨"%96"⟩;Code.part41;dropfelt ⟨"%37"⟩;dropfelt ⟨"%97"⟩;dropfelt ⟨"%98"⟩;dropfelt ⟨"%99"⟩;Code.part42;dropfelt ⟨"%40"⟩;dropfelt ⟨"%100"⟩;dropfelt ⟨"%101"⟩;dropfelt ⟨"%102"⟩;Code.part43;dropfelt ⟨"%43"⟩;dropfelt ⟨"%103"⟩;dropfelt ⟨"%104"⟩;dropfelt ⟨"%105"⟩;Code.part44;dropfelt ⟨"%46"⟩;dropfelt ⟨"%106"⟩;dropfelt ⟨"%107"⟩;dropfelt ⟨"%108"⟩;Code.part45;dropfelt ⟨"%49"⟩;dropfelt ⟨"%109"⟩;dropfelt ⟨"%110"⟩;dropfelt ⟨"%111"⟩;Code.part46;dropfelt ⟨"%52"⟩;dropfelt ⟨"%112"⟩;dropfelt ⟨"%113"⟩;dropfelt ⟨"%114"⟩;Code.part47;dropfelt ⟨"%55"⟩;dropfelt ⟨"%115"⟩;dropfelt ⟨"%116"⟩;dropfelt ⟨"%117"⟩;Code.part48;dropfelt ⟨"%58"⟩;dropfelt ⟨"%118"⟩;dropfelt ⟨"%119"⟩;dropfelt ⟨"%120"⟩;Code.part49;dropfelt ⟨"%61"⟩;dropfelt ⟨"%121"⟩;dropfelt ⟨"%122"⟩;dropfelt ⟨"%123"⟩;Code.part50;dropfelt ⟨"%64"⟩;dropfelt ⟨"%124"⟩;dropfelt ⟨"%125"⟩;dropfelt ⟨"%126"⟩;Code.part51;dropfelt ⟨"%67"⟩;dropfelt ⟨"%127"⟩;dropfelt ⟨"%128"⟩;dropfelt ⟨"%129"⟩;Code.part52;dropfelt ⟨"%70"⟩;dropfelt ⟨"%130"⟩;dropfelt ⟨"%131"⟩;dropfelt ⟨"%132"⟩;Code.part53;dropfelt ⟨"%73"⟩;dropfelt ⟨"%133"⟩;dropfelt ⟨"%134"⟩;dropfelt ⟨"%135"⟩;Code.part54;dropfelt ⟨"%18"⟩;dropfelt ⟨"%136"⟩;dropfelt ⟨"%137"⟩;dropfelt ⟨"%19"⟩) st) = [y0, y1, y2, y3, y4, y5, y6, y7, y8, y9, y10, y11, y12, y13, y14, y15, y16, y17, y18, y19] ↔
   Code.getReturn (part19_state_update st) = [y0, y1, y2, y3, y4, y5, y6, y7, y8, y9, y10, y11, y12, y13, y14, y15, y16, y17, y18, y19] := by
   unfold MLIR.runProgram; simp only
-  generalize eq : (Code.part20; Code.part21; Code.part22; Code.part23; Code.part24; Code.part25; Code.part26; Code.part27; Code.part28; Code.part29; Code.part30; Code.part31; Code.part32; Code.part33; Code.part34; Code.part35; Code.part36; Code.part37; Code.part38; Code.part39; Code.part40; Code.part41; Code.part42; Code.part43; Code.part44; Code.part45; Code.part46; Code.part47; Code.part48; Code.part49; Code.part50; Code.part51; Code.part52; Code.part53; Code.part54) = prog
+  generalize eq : (dropfelt ⟨"%175"⟩;dropfelt ⟨"%176"⟩;Code.part20;dropfelt ⟨"%17"⟩;dropfelt ⟨"%23"⟩;Code.part21;dropfelt ⟨"%16"⟩;dropfelt ⟨"%15"⟩;dropfelt ⟨"%24"⟩;dropfelt ⟨"%26"⟩;Code.part22;dropfelt ⟨"%14"⟩;dropfelt ⟨"%27"⟩;dropfelt ⟨"%29"⟩;dropfelt ⟨"%30"⟩;dropfelt ⟨"%32"⟩;Code.part23;dropfelt ⟨"%13"⟩;dropfelt ⟨"%33"⟩;dropfelt ⟨"%35"⟩;Code.part24;dropfelt ⟨"%12"⟩;dropfelt ⟨"%11"⟩;dropfelt ⟨"%36"⟩;dropfelt ⟨"%38"⟩;Code.part25;dropfelt ⟨"%10"⟩;dropfelt ⟨"%39"⟩;dropfelt ⟨"%41"⟩;dropfelt ⟨"%42"⟩;dropfelt ⟨"%44"⟩;Code.part26;dropfelt ⟨"%9"⟩;dropfelt ⟨"%45"⟩;dropfelt ⟨"%47"⟩;Code.part27;dropfelt ⟨"%8"⟩;dropfelt ⟨"%7"⟩;dropfelt ⟨"%48"⟩;dropfelt ⟨"%50"⟩;Code.part28;dropfelt ⟨"%6"⟩;dropfelt ⟨"%51"⟩;dropfelt ⟨"%53"⟩;dropfelt ⟨"%54"⟩;dropfelt ⟨"%56"⟩;Code.part29;dropfelt ⟨"%5"⟩;dropfelt ⟨"%57"⟩;dropfelt ⟨"%59"⟩;Code.part30;dropfelt ⟨"%4"⟩;dropfelt ⟨"%3"⟩;dropfelt ⟨"%60"⟩;dropfelt ⟨"%62"⟩;Code.part31;dropfelt ⟨"%2"⟩;dropfelt ⟨"%63"⟩;dropfelt ⟨"%65"⟩;dropfelt ⟨"%66"⟩;dropfelt ⟨"%68"⟩;Code.part32;dropfelt ⟨"%1"⟩;dropfelt ⟨"%69"⟩;dropfelt ⟨"%71"⟩;Code.part33;dropfelt ⟨"%20"⟩;dropfelt ⟨"%0"⟩;dropfelt ⟨"%72"⟩;dropfelt ⟨"%74"⟩;dropfelt ⟨"%75"⟩;dropfelt ⟨"%76"⟩;Code.part34;dropfelt ⟨"%78"⟩;dropfelt ⟨"%79"⟩;Code.part35;dropfelt ⟨"%21"⟩;dropfelt ⟨"%77"⟩;dropfelt ⟨"%80"⟩;dropfelt ⟨"%81"⟩;Code.part36;dropfelt ⟨"%22"⟩;dropfelt ⟨"%82"⟩;dropfelt ⟨"%83"⟩;dropfelt ⟨"%84"⟩;Code.part37;dropfelt ⟨"%25"⟩;dropfelt ⟨"%85"⟩;dropfelt ⟨"%86"⟩;dropfelt ⟨"%87"⟩;Code.part38;dropfelt ⟨"%28"⟩;dropfelt ⟨"%88"⟩;dropfelt ⟨"%89"⟩;dropfelt ⟨"%90"⟩;Code.part39;dropfelt ⟨"%31"⟩;dropfelt ⟨"%91"⟩;dropfelt ⟨"%92"⟩;dropfelt ⟨"%93"⟩;Code.part40;dropfelt ⟨"%34"⟩;dropfelt ⟨"%94"⟩;dropfelt ⟨"%95"⟩;dropfelt ⟨"%96"⟩;Code.part41;dropfelt ⟨"%37"⟩;dropfelt ⟨"%97"⟩;dropfelt ⟨"%98"⟩;dropfelt ⟨"%99"⟩;Code.part42;dropfelt ⟨"%40"⟩;dropfelt ⟨"%100"⟩;dropfelt ⟨"%101"⟩;dropfelt ⟨"%102"⟩;Code.part43;dropfelt ⟨"%43"⟩;dropfelt ⟨"%103"⟩;dropfelt ⟨"%104"⟩;dropfelt ⟨"%105"⟩;Code.part44;dropfelt ⟨"%46"⟩;dropfelt ⟨"%106"⟩;dropfelt ⟨"%107"⟩;dropfelt ⟨"%108"⟩;Code.part45;dropfelt ⟨"%49"⟩;dropfelt ⟨"%109"⟩;dropfelt ⟨"%110"⟩;dropfelt ⟨"%111"⟩;Code.part46;dropfelt ⟨"%52"⟩;dropfelt ⟨"%112"⟩;dropfelt ⟨"%113"⟩;dropfelt ⟨"%114"⟩;Code.part47;dropfelt ⟨"%55"⟩;dropfelt ⟨"%115"⟩;dropfelt ⟨"%116"⟩;dropfelt ⟨"%117"⟩;Code.part48;dropfelt ⟨"%58"⟩;dropfelt ⟨"%118"⟩;dropfelt ⟨"%119"⟩;dropfelt ⟨"%120"⟩;Code.part49;dropfelt ⟨"%61"⟩;dropfelt ⟨"%121"⟩;dropfelt ⟨"%122"⟩;dropfelt ⟨"%123"⟩;Code.part50;dropfelt ⟨"%64"⟩;dropfelt ⟨"%124"⟩;dropfelt ⟨"%125"⟩;dropfelt ⟨"%126"⟩;Code.part51;dropfelt ⟨"%67"⟩;dropfelt ⟨"%127"⟩;dropfelt ⟨"%128"⟩;dropfelt ⟨"%129"⟩;Code.part52;dropfelt ⟨"%70"⟩;dropfelt ⟨"%130"⟩;dropfelt ⟨"%131"⟩;dropfelt ⟨"%132"⟩;Code.part53;dropfelt ⟨"%73"⟩;dropfelt ⟨"%133"⟩;dropfelt ⟨"%134"⟩;dropfelt ⟨"%135"⟩;Code.part54;dropfelt ⟨"%18"⟩;dropfelt ⟨"%136"⟩;dropfelt ⟨"%137"⟩;dropfelt ⟨"%19"⟩) = prog
   unfold Code.part19
   MLIR
   rewrite [←eq]
-  unfold part19_state_update part19_state
+  rewrite [MLIR.run_seq_def,MLIR.run_dropfelt, MLIR.run_seq_def,MLIR.run_dropfelt]
+  unfold part19_state_update part19_drops part19_state
   rfl
 
 lemma part19_updates_opaque {st : State} : 
   Code.getReturn (part18_state_update st) = [y0, y1, y2, y3, y4, y5, y6, y7, y8, y9, y10, y11, y12, y13, y14, y15, y16, y17, y18, y19] ↔
-  Code.getReturn (part19_state_update (part18_state st)) = [y0, y1, y2, y3, y4, y5, y6, y7, y8, y9, y10, y11, y12, y13, y14, y15, y16, y17, y18, y19] := by
+  Code.getReturn (part19_state_update (part18_drops (part18_state st))) = [y0, y1, y2, y3, y4, y5, y6, y7, y8, y9, y10, y11, y12, y13, y14, y15, y16, y17, y18, y19] := by
   simp [part18_state_update, part19_wp]
+
+lemma part19_cumulative_wp {x0: Felt} :
+  Code.run (start_state [x0]) = [y0,y1,y2,y3,y4,y5,y6,y7,y8,y9,y10,y11,y12,y13,y14,y15,y16,y17,y18,y19] ↔
+  Code.getReturn
+        (part19_state_update
+          ({
+              buffers :=
+                (Map.empty[{ name := "code" }] ←ₘ [[some x0]])[{ name := "data" }] ←ₘ
+                  [[some (if x0 = 0 then 1 else 0), some (if x0 - 1 = 0 then 1 else 0),
+                      some (if x0 - 2 = 0 then 1 else 0), some (if x0 - 3 = 0 then 1 else 0),
+                      some (if x0 - 4 = 0 then 1 else 0), some (if x0 - 5 = 0 then 1 else 0),
+                      some (if x0 - 6 = 0 then 1 else 0), some (if x0 - 7 = 0 then 1 else 0),
+                      some (if x0 - 8 = 0 then 1 else 0), some (if x0 - 9 = 0 then 1 else 0),
+                      some (if x0 - 10 = 0 then 1 else 0), some (if x0 - 11 = 0 then 1 else 0),
+                      some (if x0 - 12 = 0 then 1 else 0), some (if x0 - 13 = 0 then 1 else 0),
+                      some (if x0 - 14 = 0 then 1 else 0), some (if x0 - 15 = 0 then 1 else 0),
+                      some (if x0 - 16 = 0 then 1 else 0), some (if x0 - 17 = 0 then 1 else 0),
+                      some (if x0 - 18 = 0 then 1 else 0), none]],
+              bufferWidths := ((fun x => Map.empty x)[{ name := "data" }] ←ₘ 20)[{ name := "code" }] ←ₘ 1,
+              constraints := [], cycle := 0,
+              felts :=
+                ((((((((((((((((((Map.empty[{ name := "%20" }] ←ₘ x0)[{ name := "%18" }] ←ₘ 1)[{ name := "%17" }] ←ₘ
+                                                  2)[{ name := "%16" }] ←ₘ
+                                                3)[{ name := "%15" }] ←ₘ
+                                              4)[{ name := "%14" }] ←ₘ
+                                            5)[{ name := "%13" }] ←ₘ
+                                          6)[{ name := "%12" }] ←ₘ
+                                        7)[{ name := "%11" }] ←ₘ
+                                      8)[{ name := "%10" }] ←ₘ
+                                    9)[{ name := "%9" }] ←ₘ
+                                  10)[{ name := "%8" }] ←ₘ
+                                11)[{ name := "%7" }] ←ₘ
+                              12)[{ name := "%6" }] ←ₘ
+                            13)[{ name := "%5" }] ←ₘ
+                          14)[{ name := "%4" }] ←ₘ
+                        15)[{ name := "%3" }] ←ₘ
+                      16)[{ name := "%2" }] ←ₘ
+                    17)[{ name := "%1" }] ←ₘ
+                  18,
+              isFailed := false, props := Map.empty,
+              vars := [{ name := "code" }, { name := "data" }] }[felts][{ name := "%0" }] ←
+            19)) =
+      [y0, y1, y2, y3, y4, y5, y6, y7, y8, y9, y10, y11, y12, y13, y14, y15, y16, y17, y18, y19]  := by
+    rewrite [part18_cumulative_wp]
+    rewrite [part19_updates_opaque]
+    unfold part18_state
+    MLIR_states_updates
+    -- 0 withEqZeros
+    -- rewrite [withEqZero_def]
+    -- MLIR_states_updates
+    unfold part18_drops
+    -- 2 drops
+    simp only [State.drop_update_swap, State.drop_update_same]
+    rewrite [State.dropFelts]
+    simp only [State.dropFelts_buffers, State.dropFelts_bufferWidths, State.dropFelts_constraints, State.dropFelts_cycle, State.dropFelts_felts, State.dropFelts_isFailed, State.dropFelts_props, State.dropFelts_vars]
+    simp only [Map.drop_base, ne_eq, Map.update_drop_swap, Map.update_drop]
+    -- 1 set
+    rewrite [Map.drop_of_updates]
+    simp only [Map.drop_base, ne_eq, Map.update_drop_swap, Map.update_drop]
 
 end Risc0.OneHot20.Witness.WP
