Risc0/Gadgets/OneHot20/Witness/WeakestPresPart7.lean
@@ -10,41 +10,88 @@ open MLIRNotation
 -- The state obtained by running Code.part7 on st
 def part7_state (st: State) : State :=
   
-          (State.set!
-            ((State.set! st { name := "data" } 2
-                  (Option.get! st.felts[({ name := "%142" }: FeltVar)]!)[felts][{ name := "%143" }] ←
-                Option.get! (State.felts st { name := "%20" }) -
-                  Option.get! (State.felts st { name := "%16" }))[felts][{ name := "%144" }] ←
-              if
-                  Option.get! (State.felts st { name := "%20" }) - Option.get! (State.felts st { name := "%16" }) =
+          ((State.set!
+              ((st[felts][{ name := "%151" }] ←
+                  Option.get! (State.felts st { name := "%20" }) -
+                    Option.get! (State.felts st { name := "%12" }))[felts][{ name := "%152" }] ←
+                if
+                    Option.get! (State.felts st { name := "%20" }) - Option.get! (State.felts st { name := "%12" }) =
+                      0 then
+                  1
+                else 0)
+              { name := "data" } 7
+              (if
+                  Option.get! (State.felts st { name := "%20" }) - Option.get! (State.felts st { name := "%12" }) =
                     0 then
                 1
-              else 0)
-            { name := "data" } 3
-            (if Option.get! (State.felts st { name := "%20" }) - Option.get! (State.felts st { name := "%16" }) = 0 then
-              1
-            else
-              0)) 
+              else 0))[felts][{ name := "%11" }] ←
+            8) 
+
+def part7_drops (st: State) : State :=
+  State.dropFelts (State.dropFelts (st) ⟨"%151"⟩) ⟨"%152"⟩
 
 -- Run the program from part7 onwards by using part7_state rather than Code.part7
 def part7_state_update (st: State): State :=
-  Γ (part7_state st) ⟦Code.part8; Code.part9; Code.part10; Code.part11; Code.part12; Code.part13; Code.part14; Code.part15; Code.part16; Code.part17; Code.part18; Code.part19; Code.part20; Code.part21; Code.part22; Code.part23; Code.part24; Code.part25; Code.part26; Code.part27; Code.part28; Code.part29; Code.part30; Code.part31; Code.part32; Code.part33; Code.part34; Code.part35; Code.part36; Code.part37; Code.part38; Code.part39; Code.part40; Code.part41; Code.part42; Code.part43; Code.part44; Code.part45; Code.part46; Code.part47; Code.part48; Code.part49; Code.part50; Code.part51; Code.part52; Code.part53; Code.part54⟧
+  Γ (part7_drops (part7_state st)) ⟦Code.part8;dropfelt ⟨"%153"⟩;dropfelt ⟨"%154"⟩;Code.part9;dropfelt ⟨"%155"⟩;dropfelt ⟨"%156"⟩;Code.part10;dropfelt ⟨"%157"⟩;dropfelt ⟨"%158"⟩;Code.part11;dropfelt ⟨"%159"⟩;dropfelt ⟨"%160"⟩;Code.part12;dropfelt ⟨"%161"⟩;dropfelt ⟨"%162"⟩;Code.part13;dropfelt ⟨"%163"⟩;dropfelt ⟨"%164"⟩;Code.part14;dropfelt ⟨"%165"⟩;dropfelt ⟨"%166"⟩;Code.part15;dropfelt ⟨"%167"⟩;dropfelt ⟨"%168"⟩;Code.part16;dropfelt ⟨"%169"⟩;dropfelt ⟨"%170"⟩;Code.part17;dropfelt ⟨"%171"⟩;dropfelt ⟨"%172"⟩;Code.part18;dropfelt ⟨"%173"⟩;dropfelt ⟨"%174"⟩;Code.part19;dropfelt ⟨"%175"⟩;dropfelt ⟨"%176"⟩;Code.part20;dropfelt ⟨"%17"⟩;dropfelt ⟨"%23"⟩;Code.part21;dropfelt ⟨"%16"⟩;dropfelt ⟨"%15"⟩;dropfelt ⟨"%24"⟩;dropfelt ⟨"%26"⟩;Code.part22;dropfelt ⟨"%14"⟩;dropfelt ⟨"%27"⟩;dropfelt ⟨"%29"⟩;dropfelt ⟨"%30"⟩;dropfelt ⟨"%32"⟩;Code.part23;dropfelt ⟨"%13"⟩;dropfelt ⟨"%33"⟩;dropfelt ⟨"%35"⟩;Code.part24;dropfelt ⟨"%12"⟩;dropfelt ⟨"%11"⟩;dropfelt ⟨"%36"⟩;dropfelt ⟨"%38"⟩;Code.part25;dropfelt ⟨"%10"⟩;dropfelt ⟨"%39"⟩;dropfelt ⟨"%41"⟩;dropfelt ⟨"%42"⟩;dropfelt ⟨"%44"⟩;Code.part26;dropfelt ⟨"%9"⟩;dropfelt ⟨"%45"⟩;dropfelt ⟨"%47"⟩;Code.part27;dropfelt ⟨"%8"⟩;dropfelt ⟨"%7"⟩;dropfelt ⟨"%48"⟩;dropfelt ⟨"%50"⟩;Code.part28;dropfelt ⟨"%6"⟩;dropfelt ⟨"%51"⟩;dropfelt ⟨"%53"⟩;dropfelt ⟨"%54"⟩;dropfelt ⟨"%56"⟩;Code.part29;dropfelt ⟨"%5"⟩;dropfelt ⟨"%57"⟩;dropfelt ⟨"%59"⟩;Code.part30;dropfelt ⟨"%4"⟩;dropfelt ⟨"%3"⟩;dropfelt ⟨"%60"⟩;dropfelt ⟨"%62"⟩;Code.part31;dropfelt ⟨"%2"⟩;dropfelt ⟨"%63"⟩;dropfelt ⟨"%65"⟩;dropfelt ⟨"%66"⟩;dropfelt ⟨"%68"⟩;Code.part32;dropfelt ⟨"%1"⟩;dropfelt ⟨"%69"⟩;dropfelt ⟨"%71"⟩;Code.part33;dropfelt ⟨"%20"⟩;dropfelt ⟨"%0"⟩;dropfelt ⟨"%72"⟩;dropfelt ⟨"%74"⟩;dropfelt ⟨"%75"⟩;dropfelt ⟨"%76"⟩;Code.part34;dropfelt ⟨"%78"⟩;dropfelt ⟨"%79"⟩;Code.part35;dropfelt ⟨"%21"⟩;dropfelt ⟨"%77"⟩;dropfelt ⟨"%80"⟩;dropfelt ⟨"%81"⟩;Code.part36;dropfelt ⟨"%22"⟩;dropfelt ⟨"%82"⟩;dropfelt ⟨"%83"⟩;dropfelt ⟨"%84"⟩;Code.part37;dropfelt ⟨"%25"⟩;dropfelt ⟨"%85"⟩;dropfelt ⟨"%86"⟩;dropfelt ⟨"%87"⟩;Code.part38;dropfelt ⟨"%28"⟩;dropfelt ⟨"%88"⟩;dropfelt ⟨"%89"⟩;dropfelt ⟨"%90"⟩;Code.part39;dropfelt ⟨"%31"⟩;dropfelt ⟨"%91"⟩;dropfelt ⟨"%92"⟩;dropfelt ⟨"%93"⟩;Code.part40;dropfelt ⟨"%34"⟩;dropfelt ⟨"%94"⟩;dropfelt ⟨"%95"⟩;dropfelt ⟨"%96"⟩;Code.part41;dropfelt ⟨"%37"⟩;dropfelt ⟨"%97"⟩;dropfelt ⟨"%98"⟩;dropfelt ⟨"%99"⟩;Code.part42;dropfelt ⟨"%40"⟩;dropfelt ⟨"%100"⟩;dropfelt ⟨"%101"⟩;dropfelt ⟨"%102"⟩;Code.part43;dropfelt ⟨"%43"⟩;dropfelt ⟨"%103"⟩;dropfelt ⟨"%104"⟩;dropfelt ⟨"%105"⟩;Code.part44;dropfelt ⟨"%46"⟩;dropfelt ⟨"%106"⟩;dropfelt ⟨"%107"⟩;dropfelt ⟨"%108"⟩;Code.part45;dropfelt ⟨"%49"⟩;dropfelt ⟨"%109"⟩;dropfelt ⟨"%110"⟩;dropfelt ⟨"%111"⟩;Code.part46;dropfelt ⟨"%52"⟩;dropfelt ⟨"%112"⟩;dropfelt ⟨"%113"⟩;dropfelt ⟨"%114"⟩;Code.part47;dropfelt ⟨"%55"⟩;dropfelt ⟨"%115"⟩;dropfelt ⟨"%116"⟩;dropfelt ⟨"%117"⟩;Code.part48;dropfelt ⟨"%58"⟩;dropfelt ⟨"%118"⟩;dropfelt ⟨"%119"⟩;dropfelt ⟨"%120"⟩;Code.part49;dropfelt ⟨"%61"⟩;dropfelt ⟨"%121"⟩;dropfelt ⟨"%122"⟩;dropfelt ⟨"%123"⟩;Code.part50;dropfelt ⟨"%64"⟩;dropfelt ⟨"%124"⟩;dropfelt ⟨"%125"⟩;dropfelt ⟨"%126"⟩;Code.part51;dropfelt ⟨"%67"⟩;dropfelt ⟨"%127"⟩;dropfelt ⟨"%128"⟩;dropfelt ⟨"%129"⟩;Code.part52;dropfelt ⟨"%70"⟩;dropfelt ⟨"%130"⟩;dropfelt ⟨"%131"⟩;dropfelt ⟨"%132"⟩;Code.part53;dropfelt ⟨"%73"⟩;dropfelt ⟨"%133"⟩;dropfelt ⟨"%134"⟩;dropfelt ⟨"%135"⟩;Code.part54;dropfelt ⟨"%18"⟩;dropfelt ⟨"%136"⟩;dropfelt ⟨"%137"⟩;dropfelt ⟨"%19"⟩⟧
 
 -- Prove that substituting part7_state for Code.part7 produces the same result
 lemma part7_wp {st : State} {y0 y1 y2 y3 y4 y5 y6 y7 y8 y9 y10 y11 y12 y13 y14 y15 y16 y17 y18 y19 : Option Felt} :
-  Code.getReturn (MLIR.runProgram (Code.part7; Code.part8; Code.part9; Code.part10; Code.part11; Code.part12; Code.part13; Code.part14; Code.part15; Code.part16; Code.part17; Code.part18; Code.part19; Code.part20; Code.part21; Code.part22; Code.part23; Code.part24; Code.part25; Code.part26; Code.part27; Code.part28; Code.part29; Code.part30; Code.part31; Code.part32; Code.part33; Code.part34; Code.part35; Code.part36; Code.part37; Code.part38; Code.part39; Code.part40; Code.part41; Code.part42; Code.part43; Code.part44; Code.part45; Code.part46; Code.part47; Code.part48; Code.part49; Code.part50; Code.part51; Code.part52; Code.part53; Code.part54) st) = [y0, y1, y2, y3, y4, y5, y6, y7, y8, y9, y10, y11, y12, y13, y14, y15, y16, y17, y18, y19] ↔
+  Code.getReturn (MLIR.runProgram (Code.part7;dropfelt ⟨"%151"⟩;dropfelt ⟨"%152"⟩;Code.part8;dropfelt ⟨"%153"⟩;dropfelt ⟨"%154"⟩;Code.part9;dropfelt ⟨"%155"⟩;dropfelt ⟨"%156"⟩;Code.part10;dropfelt ⟨"%157"⟩;dropfelt ⟨"%158"⟩;Code.part11;dropfelt ⟨"%159"⟩;dropfelt ⟨"%160"⟩;Code.part12;dropfelt ⟨"%161"⟩;dropfelt ⟨"%162"⟩;Code.part13;dropfelt ⟨"%163"⟩;dropfelt ⟨"%164"⟩;Code.part14;dropfelt ⟨"%165"⟩;dropfelt ⟨"%166"⟩;Code.part15;dropfelt ⟨"%167"⟩;dropfelt ⟨"%168"⟩;Code.part16;dropfelt ⟨"%169"⟩;dropfelt ⟨"%170"⟩;Code.part17;dropfelt ⟨"%171"⟩;dropfelt ⟨"%172"⟩;Code.part18;dropfelt ⟨"%173"⟩;dropfelt ⟨"%174"⟩;Code.part19;dropfelt ⟨"%175"⟩;dropfelt ⟨"%176"⟩;Code.part20;dropfelt ⟨"%17"⟩;dropfelt ⟨"%23"⟩;Code.part21;dropfelt ⟨"%16"⟩;dropfelt ⟨"%15"⟩;dropfelt ⟨"%24"⟩;dropfelt ⟨"%26"⟩;Code.part22;dropfelt ⟨"%14"⟩;dropfelt ⟨"%27"⟩;dropfelt ⟨"%29"⟩;dropfelt ⟨"%30"⟩;dropfelt ⟨"%32"⟩;Code.part23;dropfelt ⟨"%13"⟩;dropfelt ⟨"%33"⟩;dropfelt ⟨"%35"⟩;Code.part24;dropfelt ⟨"%12"⟩;dropfelt ⟨"%11"⟩;dropfelt ⟨"%36"⟩;dropfelt ⟨"%38"⟩;Code.part25;dropfelt ⟨"%10"⟩;dropfelt ⟨"%39"⟩;dropfelt ⟨"%41"⟩;dropfelt ⟨"%42"⟩;dropfelt ⟨"%44"⟩;Code.part26;dropfelt ⟨"%9"⟩;dropfelt ⟨"%45"⟩;dropfelt ⟨"%47"⟩;Code.part27;dropfelt ⟨"%8"⟩;dropfelt ⟨"%7"⟩;dropfelt ⟨"%48"⟩;dropfelt ⟨"%50"⟩;Code.part28;dropfelt ⟨"%6"⟩;dropfelt ⟨"%51"⟩;dropfelt ⟨"%53"⟩;dropfelt ⟨"%54"⟩;dropfelt ⟨"%56"⟩;Code.part29;dropfelt ⟨"%5"⟩;dropfelt ⟨"%57"⟩;dropfelt ⟨"%59"⟩;Code.part30;dropfelt ⟨"%4"⟩;dropfelt ⟨"%3"⟩;dropfelt ⟨"%60"⟩;dropfelt ⟨"%62"⟩;Code.part31;dropfelt ⟨"%2"⟩;dropfelt ⟨"%63"⟩;dropfelt ⟨"%65"⟩;dropfelt ⟨"%66"⟩;dropfelt ⟨"%68"⟩;Code.part32;dropfelt ⟨"%1"⟩;dropfelt ⟨"%69"⟩;dropfelt ⟨"%71"⟩;Code.part33;dropfelt ⟨"%20"⟩;dropfelt ⟨"%0"⟩;dropfelt ⟨"%72"⟩;dropfelt ⟨"%74"⟩;dropfelt ⟨"%75"⟩;dropfelt ⟨"%76"⟩;Code.part34;dropfelt ⟨"%78"⟩;dropfelt ⟨"%79"⟩;Code.part35;dropfelt ⟨"%21"⟩;dropfelt ⟨"%77"⟩;dropfelt ⟨"%80"⟩;dropfelt ⟨"%81"⟩;Code.part36;dropfelt ⟨"%22"⟩;dropfelt ⟨"%82"⟩;dropfelt ⟨"%83"⟩;dropfelt ⟨"%84"⟩;Code.part37;dropfelt ⟨"%25"⟩;dropfelt ⟨"%85"⟩;dropfelt ⟨"%86"⟩;dropfelt ⟨"%87"⟩;Code.part38;dropfelt ⟨"%28"⟩;dropfelt ⟨"%88"⟩;dropfelt ⟨"%89"⟩;dropfelt ⟨"%90"⟩;Code.part39;dropfelt ⟨"%31"⟩;dropfelt ⟨"%91"⟩;dropfelt ⟨"%92"⟩;dropfelt ⟨"%93"⟩;Code.part40;dropfelt ⟨"%34"⟩;dropfelt ⟨"%94"⟩;dropfelt ⟨"%95"⟩;dropfelt ⟨"%96"⟩;Code.part41;dropfelt ⟨"%37"⟩;dropfelt ⟨"%97"⟩;dropfelt ⟨"%98"⟩;dropfelt ⟨"%99"⟩;Code.part42;dropfelt ⟨"%40"⟩;dropfelt ⟨"%100"⟩;dropfelt ⟨"%101"⟩;dropfelt ⟨"%102"⟩;Code.part43;dropfelt ⟨"%43"⟩;dropfelt ⟨"%103"⟩;dropfelt ⟨"%104"⟩;dropfelt ⟨"%105"⟩;Code.part44;dropfelt ⟨"%46"⟩;dropfelt ⟨"%106"⟩;dropfelt ⟨"%107"⟩;dropfelt ⟨"%108"⟩;Code.part45;dropfelt ⟨"%49"⟩;dropfelt ⟨"%109"⟩;dropfelt ⟨"%110"⟩;dropfelt ⟨"%111"⟩;Code.part46;dropfelt ⟨"%52"⟩;dropfelt ⟨"%112"⟩;dropfelt ⟨"%113"⟩;dropfelt ⟨"%114"⟩;Code.part47;dropfelt ⟨"%55"⟩;dropfelt ⟨"%115"⟩;dropfelt ⟨"%116"⟩;dropfelt ⟨"%117"⟩;Code.part48;dropfelt ⟨"%58"⟩;dropfelt ⟨"%118"⟩;dropfelt ⟨"%119"⟩;dropfelt ⟨"%120"⟩;Code.part49;dropfelt ⟨"%61"⟩;dropfelt ⟨"%121"⟩;dropfelt ⟨"%122"⟩;dropfelt ⟨"%123"⟩;Code.part50;dropfelt ⟨"%64"⟩;dropfelt ⟨"%124"⟩;dropfelt ⟨"%125"⟩;dropfelt ⟨"%126"⟩;Code.part51;dropfelt ⟨"%67"⟩;dropfelt ⟨"%127"⟩;dropfelt ⟨"%128"⟩;dropfelt ⟨"%129"⟩;Code.part52;dropfelt ⟨"%70"⟩;dropfelt ⟨"%130"⟩;dropfelt ⟨"%131"⟩;dropfelt ⟨"%132"⟩;Code.part53;dropfelt ⟨"%73"⟩;dropfelt ⟨"%133"⟩;dropfelt ⟨"%134"⟩;dropfelt ⟨"%135"⟩;Code.part54;dropfelt ⟨"%18"⟩;dropfelt ⟨"%136"⟩;dropfelt ⟨"%137"⟩;dropfelt ⟨"%19"⟩) st) = [y0, y1, y2, y3, y4, y5, y6, y7, y8, y9, y10, y11, y12, y13, y14, y15, y16, y17, y18, y19] ↔
   Code.getReturn (part7_state_update st) = [y0, y1, y2, y3, y4, y5, y6, y7, y8, y9, y10, y11, y12, y13, y14, y15, y16, y17, y18, y19] := by
   unfold MLIR.runProgram; simp only
-  generalize eq : (Code.part8; Code.part9; Code.part10; Code.part11; Code.part12; Code.part13; Code.part14; Code.part15; Code.part16; Code.part17; Code.part18; Code.part19; Code.part20; Code.part21; Code.part22; Code.part23; Code.part24; Code.part25; Code.part26; Code.part27; Code.part28; Code.part29; Code.part30; Code.part31; Code.part32; Code.part33; Code.part34; Code.part35; Code.part36; Code.part37; Code.part38; Code.part39; Code.part40; Code.part41; Code.part42; Code.part43; Code.part44; Code.part45; Code.part46; Code.part47; Code.part48; Code.part49; Code.part50; Code.part51; Code.part52; Code.part53; Code.part54) = prog
+  generalize eq : (dropfelt ⟨"%151"⟩;dropfelt ⟨"%152"⟩;Code.part8;dropfelt ⟨"%153"⟩;dropfelt ⟨"%154"⟩;Code.part9;dropfelt ⟨"%155"⟩;dropfelt ⟨"%156"⟩;Code.part10;dropfelt ⟨"%157"⟩;dropfelt ⟨"%158"⟩;Code.part11;dropfelt ⟨"%159"⟩;dropfelt ⟨"%160"⟩;Code.part12;dropfelt ⟨"%161"⟩;dropfelt ⟨"%162"⟩;Code.part13;dropfelt ⟨"%163"⟩;dropfelt ⟨"%164"⟩;Code.part14;dropfelt ⟨"%165"⟩;dropfelt ⟨"%166"⟩;Code.part15;dropfelt ⟨"%167"⟩;dropfelt ⟨"%168"⟩;Code.part16;dropfelt ⟨"%169"⟩;dropfelt ⟨"%170"⟩;Code.part17;dropfelt ⟨"%171"⟩;dropfelt ⟨"%172"⟩;Code.part18;dropfelt ⟨"%173"⟩;dropfelt ⟨"%174"⟩;Code.part19;dropfelt ⟨"%175"⟩;dropfelt ⟨"%176"⟩;Code.part20;dropfelt ⟨"%17"⟩;dropfelt ⟨"%23"⟩;Code.part21;dropfelt ⟨"%16"⟩;dropfelt ⟨"%15"⟩;dropfelt ⟨"%24"⟩;dropfelt ⟨"%26"⟩;Code.part22;dropfelt ⟨"%14"⟩;dropfelt ⟨"%27"⟩;dropfelt ⟨"%29"⟩;dropfelt ⟨"%30"⟩;dropfelt ⟨"%32"⟩;Code.part23;dropfelt ⟨"%13"⟩;dropfelt ⟨"%33"⟩;dropfelt ⟨"%35"⟩;Code.part24;dropfelt ⟨"%12"⟩;dropfelt ⟨"%11"⟩;dropfelt ⟨"%36"⟩;dropfelt ⟨"%38"⟩;Code.part25;dropfelt ⟨"%10"⟩;dropfelt ⟨"%39"⟩;dropfelt ⟨"%41"⟩;dropfelt ⟨"%42"⟩;dropfelt ⟨"%44"⟩;Code.part26;dropfelt ⟨"%9"⟩;dropfelt ⟨"%45"⟩;dropfelt ⟨"%47"⟩;Code.part27;dropfelt ⟨"%8"⟩;dropfelt ⟨"%7"⟩;dropfelt ⟨"%48"⟩;dropfelt ⟨"%50"⟩;Code.part28;dropfelt ⟨"%6"⟩;dropfelt ⟨"%51"⟩;dropfelt ⟨"%53"⟩;dropfelt ⟨"%54"⟩;dropfelt ⟨"%56"⟩;Code.part29;dropfelt ⟨"%5"⟩;dropfelt ⟨"%57"⟩;dropfelt ⟨"%59"⟩;Code.part30;dropfelt ⟨"%4"⟩;dropfelt ⟨"%3"⟩;dropfelt ⟨"%60"⟩;dropfelt ⟨"%62"⟩;Code.part31;dropfelt ⟨"%2"⟩;dropfelt ⟨"%63"⟩;dropfelt ⟨"%65"⟩;dropfelt ⟨"%66"⟩;dropfelt ⟨"%68"⟩;Code.part32;dropfelt ⟨"%1"⟩;dropfelt ⟨"%69"⟩;dropfelt ⟨"%71"⟩;Code.part33;dropfelt ⟨"%20"⟩;dropfelt ⟨"%0"⟩;dropfelt ⟨"%72"⟩;dropfelt ⟨"%74"⟩;dropfelt ⟨"%75"⟩;dropfelt ⟨"%76"⟩;Code.part34;dropfelt ⟨"%78"⟩;dropfelt ⟨"%79"⟩;Code.part35;dropfelt ⟨"%21"⟩;dropfelt ⟨"%77"⟩;dropfelt ⟨"%80"⟩;dropfelt ⟨"%81"⟩;Code.part36;dropfelt ⟨"%22"⟩;dropfelt ⟨"%82"⟩;dropfelt ⟨"%83"⟩;dropfelt ⟨"%84"⟩;Code.part37;dropfelt ⟨"%25"⟩;dropfelt ⟨"%85"⟩;dropfelt ⟨"%86"⟩;dropfelt ⟨"%87"⟩;Code.part38;dropfelt ⟨"%28"⟩;dropfelt ⟨"%88"⟩;dropfelt ⟨"%89"⟩;dropfelt ⟨"%90"⟩;Code.part39;dropfelt ⟨"%31"⟩;dropfelt ⟨"%91"⟩;dropfelt ⟨"%92"⟩;dropfelt ⟨"%93"⟩;Code.part40;dropfelt ⟨"%34"⟩;dropfelt ⟨"%94"⟩;dropfelt ⟨"%95"⟩;dropfelt ⟨"%96"⟩;Code.part41;dropfelt ⟨"%37"⟩;dropfelt ⟨"%97"⟩;dropfelt ⟨"%98"⟩;dropfelt ⟨"%99"⟩;Code.part42;dropfelt ⟨"%40"⟩;dropfelt ⟨"%100"⟩;dropfelt ⟨"%101"⟩;dropfelt ⟨"%102"⟩;Code.part43;dropfelt ⟨"%43"⟩;dropfelt ⟨"%103"⟩;dropfelt ⟨"%104"⟩;dropfelt ⟨"%105"⟩;Code.part44;dropfelt ⟨"%46"⟩;dropfelt ⟨"%106"⟩;dropfelt ⟨"%107"⟩;dropfelt ⟨"%108"⟩;Code.part45;dropfelt ⟨"%49"⟩;dropfelt ⟨"%109"⟩;dropfelt ⟨"%110"⟩;dropfelt ⟨"%111"⟩;Code.part46;dropfelt ⟨"%52"⟩;dropfelt ⟨"%112"⟩;dropfelt ⟨"%113"⟩;dropfelt ⟨"%114"⟩;Code.part47;dropfelt ⟨"%55"⟩;dropfelt ⟨"%115"⟩;dropfelt ⟨"%116"⟩;dropfelt ⟨"%117"⟩;Code.part48;dropfelt ⟨"%58"⟩;dropfelt ⟨"%118"⟩;dropfelt ⟨"%119"⟩;dropfelt ⟨"%120"⟩;Code.part49;dropfelt ⟨"%61"⟩;dropfelt ⟨"%121"⟩;dropfelt ⟨"%122"⟩;dropfelt ⟨"%123"⟩;Code.part50;dropfelt ⟨"%64"⟩;dropfelt ⟨"%124"⟩;dropfelt ⟨"%125"⟩;dropfelt ⟨"%126"⟩;Code.part51;dropfelt ⟨"%67"⟩;dropfelt ⟨"%127"⟩;dropfelt ⟨"%128"⟩;dropfelt ⟨"%129"⟩;Code.part52;dropfelt ⟨"%70"⟩;dropfelt ⟨"%130"⟩;dropfelt ⟨"%131"⟩;dropfelt ⟨"%132"⟩;Code.part53;dropfelt ⟨"%73"⟩;dropfelt ⟨"%133"⟩;dropfelt ⟨"%134"⟩;dropfelt ⟨"%135"⟩;Code.part54;dropfelt ⟨"%18"⟩;dropfelt ⟨"%136"⟩;dropfelt ⟨"%137"⟩;dropfelt ⟨"%19"⟩) = prog
   unfold Code.part7
   MLIR
   rewrite [←eq]
-  unfold part7_state_update part7_state
+  rewrite [MLIR.run_seq_def,MLIR.run_dropfelt, MLIR.run_seq_def,MLIR.run_dropfelt]
+  unfold part7_state_update part7_drops part7_state
   rfl
 
 lemma part7_updates_opaque {st : State} : 
   Code.getReturn (part6_state_update st) = [y0, y1, y2, y3, y4, y5, y6, y7, y8, y9, y10, y11, y12, y13, y14, y15, y16, y17, y18, y19] ↔
-  Code.getReturn (part7_state_update (part6_state st)) = [y0, y1, y2, y3, y4, y5, y6, y7, y8, y9, y10, y11, y12, y13, y14, y15, y16, y17, y18, y19] := by
+  Code.getReturn (part7_state_update (part6_drops (part6_state st))) = [y0, y1, y2, y3, y4, y5, y6, y7, y8, y9, y10, y11, y12, y13, y14, y15, y16, y17, y18, y19] := by
   simp [part6_state_update, part7_wp]
+
+lemma part7_cumulative_wp {x0: Felt} :
+  Code.run (start_state [x0]) = [y0,y1,y2,y3,y4,y5,y6,y7,y8,y9,y10,y11,y12,y13,y14,y15,y16,y17,y18,y19] ↔
+  Code.getReturn
+        (part7_state_update
+          ({
+              buffers :=
+                (Map.empty[{ name := "code" }] ←ₘ [[some x0]])[{ name := "data" }] ←ₘ
+                  [[some (if x0 = 0 then 1 else 0), some (if x0 - 1 = 0 then 1 else 0),
+                      some (if x0 - 2 = 0 then 1 else 0), some (if x0 - 3 = 0 then 1 else 0),
+                      some (if x0 - 4 = 0 then 1 else 0), some (if x0 - 5 = 0 then 1 else 0),
+                      some (if x0 - 6 = 0 then 1 else 0), none, none, none, none, none, none, none, none, none, none,
+                      none, none, none]],
+              bufferWidths := ((fun x => Map.empty x)[{ name := "data" }] ←ₘ 20)[{ name := "code" }] ←ₘ 1,
+              constraints := [], cycle := 0,
+              felts :=
+                ((((((Map.empty[{ name := "%20" }] ←ₘ x0)[{ name := "%18" }] ←ₘ 1)[{ name := "%17" }] ←ₘ
+                          2)[{ name := "%16" }] ←ₘ
+                        3)[{ name := "%15" }] ←ₘ
+                      4)[{ name := "%14" }] ←ₘ
+                    5)[{ name := "%13" }] ←ₘ
+                  6,
+              isFailed := false, props := Map.empty,
+              vars := [{ name := "code" }, { name := "data" }] }[felts][{ name := "%12" }] ←
+            7)) =
+      [y0, y1, y2, y3, y4, y5, y6, y7, y8, y9, y10, y11, y12, y13, y14, y15, y16, y17, y18, y19]  := by
+    rewrite [part6_cumulative_wp]
+    rewrite [part7_updates_opaque]
+    unfold part6_state
+    MLIR_states_updates
+    -- 0 withEqZeros
+    -- rewrite [withEqZero_def]
+    -- MLIR_states_updates
+    unfold part6_drops
+    -- 2 drops
+    simp only [State.drop_update_swap, State.drop_update_same]
+    rewrite [State.dropFelts]
+    simp only [State.dropFelts_buffers, State.dropFelts_bufferWidths, State.dropFelts_constraints, State.dropFelts_cycle, State.dropFelts_felts, State.dropFelts_isFailed, State.dropFelts_props, State.dropFelts_vars]
+    simp only [Map.drop_base, ne_eq, Map.update_drop_swap, Map.update_drop]
+    -- 1 set
+    rewrite [Map.drop_of_updates]
+    simp only [Map.drop_base, ne_eq, Map.update_drop_swap, Map.update_drop]
 
 end Risc0.OneHot20.Witness.WP
